theories/logic/ewpw.v
@@ -16,15 +16,14 @@ From hazel.program_logic Require Import weakest_precondition
 (* Local imports *)
 From haffel.lib Require Import logic.
 From haffel.lang Require Import haffel.
-From haffel.lang Require Import subst_map.
-From haffel.logic Require Import iEff.
 From haffel.logic Require Import sem_def.
+From haffel.logic Require Import mode.
 From haffel.logic Require Import sem_sig.
 From haffel.logic Require Import sem_row.
 
 (* EWP wrapper *)
 Definition ewpw `{!heapGS Σ} (E : coPset) (e : expr) (ρ : sem_row Σ) (Φ : val -d> iPropO Σ) : iPropO Σ := 
-    (EWP e @ E <| ⟦ filter_os ρ ⟧ |> {| ⟦ ρ ⟧ |} {{ Φ }})%R%I.
+    (EWP e @ E <| ⟦ filter_os ρ%R ⟧ |> {| ⟦ ρ%R ⟧ |} {{ Φ }})%R%I.
 
 Global Opaque env_dom.
 
@@ -52,25 +51,25 @@ Notation "'EWPW' e {{ Φ } }" :=
    format "'[' 'EWPW'  e  '/' '[          ' {{  Φ  } } ']' ']'") : bi_scope.
 
 Notation "'EWPW' e @ E '<|' ρ '|' '>' {{ Φ } }" :=
-  (ewpw E e%E ρ Φ)
+  (ewpw E e%E ρ%R Φ)
   (at level 20, e, ρ, Φ at level 200,
    format "'[' 'EWPW'  e  '/' '[          ' @  E '<|' ρ '|' '>' {{  Φ  } } ']' ']'") : bi_scope.
 
 (* Postcondition includes binder. *)
 Notation "'EWPW' e @ E '<|' ρ '|' '>' {{ v , Φ } }" :=
-  (ewpw E e%E ρ (λ v, Φ)%I)
+  (ewpw E e%E ρ%R (λ v, Φ)%I)
   (at level 20, e, ρ, Φ at level 200,
    format "'[' 'EWPW'  e  '/' '[          ' @  E '<|' ρ '|' '>'  {{  v ,  Φ  } } ']' ']'") : bi_scope.
 
 (* Mask is implicitly specified by ⊤. *)
 Notation "'EWPW' e '<|' ρ '|' '>' {{ v , Φ } }" :=
-  (ewpw ⊤ e%E ρ (λ v, Φ)%I)
+  (ewpw ⊤ e%E ρ%R (λ v, Φ)%I)
   (at level 20, e, ρ, Φ at level 200,
    format "'[' 'EWPW'  e  '/' '[          ' '<|' ρ '|' '>' {{  v ,  Φ  } } ']' ']'") : bi_scope.
 
 (* No binder and no mask. *)
 Notation "'EWPW' e '<|' ρ '|' '>' {{ Φ } }" :=
-  (ewpw ⊤ e%E ρ Φ%I)
+  (ewpw ⊤ e%E ρ%R Φ%I)
   (at level 20, e, ρ, Φ at level 200,
    format "'[' 'EWPW'  e  '/' '[          ' '<|' ρ '|' '>' {{  Φ  } } ']' ']'") : bi_scope.
 
@@ -95,318 +94,510 @@ Qed.
 
 Section reasoning.
 
-  Context `{!heapGS Σ}. 
+Context `{!heapGS Σ}. 
 
-  Lemma filter_os_nil :
-    filter_os (⟨⟩ : sem_row Σ)%R = (⟨⟩ : sem_row Σ)%R.
-  Proof.
-    rewrite /filter_os.
-    rewrite union_with_idemp; first done.
-    intros ?? H. rewrite lookup_empty in H. inv H.
-  Qed.
+Lemma ewpw_value (E : coPset) ρ Φ (v : val) :
+  Φ v -∗ EWPW v @E <| ρ |> {{ Φ }}.
+Proof.
+  iIntros "HΦ". rewrite /ewpw. by iApply ewp_value. 
+Qed.
 
-  Lemma ewpw_value (E : coPset) ρ Φ (v : val) :
-    Φ v -∗ EWPW v @E <| ρ |> {{ Φ }}.
-  Proof.
-    iIntros "HΦ". rewrite /ewpw. by iApply ewp_value. 
-  Qed.
-  
-  Lemma ewpw_bot E e Φ :
-    EWP e @ E {{ v, Φ v }} -∗
-    EWPW e @ E {{ Φ }}.
-  Proof. 
-    iIntros "Hewp". rewrite /ewpw /=.
-    iApply ewp_ms_prot_mono.
-    { iApply iEff_le_bottom. }
-    rewrite filter_os_nil.
-    iApply ewp_os_prot_mono.
-    { iApply iEff_le_bottom. }
-    iApply "Hewp".
-  Qed.
-  
-  Lemma ewpw_bot_inv e E Φ :
-    EWPW e @ E {{ Φ }} -∗
-    EWP e @ E {{ v, Φ v }}.
-  Proof. 
-    iIntros "Hewp".
-    rewrite /ewpw /=.
-    rewrite filter_os_nil.
-    iApply ewp_ms_prot_mono.
-    { iApply row_nil_iEff_bot. }
-    iApply ewp_os_prot_mono.
-    { iApply row_nil_iEff_bot. }
-    iApply "Hewp".
-  Qed.
-  
-  Lemma ewpw_sub E e ρ ρ' Φ :
-    ρ ≤R ρ' -∗ 
-    EWPW e @E <| ρ |> {{ Φ }} -∗ EWPW e @E <| ρ' |> {{ Φ }}. 
-  Proof.
-    iIntros "#Hρρ' Hewp".
-    rewrite /ewpw.
-    iApply ewp_ms_prot_mono; first (iApply (row_le_iEff with "Hρρ'")). 
-    iApply ewp_os_prot_mono; last done. 
-    { iApply row_le_iEff. by iApply row_le_filter_os_mono. }
-  Qed.
+Lemma ewpw_bot E e Φ :
+  EWP e @ E {{ v, Φ v }} -∗
+  EWPW e @ E {{ Φ }}.
+Proof. 
+  iIntros "Hewp". rewrite /ewpw /=.
+  iApply ewp_ms_prot_mono.
+  { iApply iEff_le_bottom. }
+  rewrite filter_os_nil.
+  iApply ewp_os_prot_mono.
+  { iApply iEff_le_bottom. }
+  iApply "Hewp".
+Qed.
 
-  Lemma ewp_mono_os E (ρ ρ' : sem_row Σ) e Φ Φ' `{! OSRow ρ } `{! OSRow ρ' } :
-    EWP e @ E <| ⟦ ρ ⟧%R |> {| ⟦ ρ' ⟧%R |} {{ v, Φ v }} -∗
-    (∀ v : val, Φ v ={E}=∗ Φ' v) -∗ EWP e @ E <| ⟦ ρ ⟧%R |> {| ⟦ ρ' ⟧%R |} {{ v, Φ' v }}.
-  Proof.
-    iIntros "Hewp Himp". 
-    iLöb as "IH" forall (e).
-    rewrite !ewp_unfold /ewp_pre.
-    destruct (to_val e) eqn:?.
-    { iMod "Hewp" as "Hewp". by iApply "Himp". }
-    destruct (to_eff e) eqn:?.
-    - simpl. destruct p eqn:?, p0 eqn:?, m;
-      iDestruct "Hewp" as "(%Φ'' & HΨ & Hps)";
-      iExists (λ w, Φ'' w ∗ (∀ v, Φ v ={E}=∗ Φ' v)%I)%I;
-      iSplitL "HΨ Himp".
-      2, 4: try (iDestruct "Hps" as "#Hps"; iModIntro);
-            iIntros "% (HΦ'' & Himp)"; 
-            iSpecialize ("Hps" with "HΦ''"); iNext;
-            iApply ("IH" with "Hps Himp").
-      + destruct OSRow0 as [];
-        iApply (monotonic_prot with "[Himp] HΨ"); iIntros "% $ {$Himp}".
-      + destruct OSRow1 as [];
-        iApply (monotonic_prot with "[Himp] HΨ"); iIntros "% $ {$Himp}".
-    - iIntros (σ₁ ns κ' κs nt) "Hstate".
-      iSpecialize ("Hewp" $! σ₁ ns κ' κs nt with "Hstate"). 
-      iMod "Hewp" as "Hewp". iModIntro.
-      iDestruct "Hewp" as "(Hred & Hpost)".
-      iFrame. iIntros (e₂ σ₂) "Hprim Hcred".
-      iSpecialize ("Hpost" $! e₂ σ₂ with "Hprim Hcred").
-      iInduction (num_laters_per_step) as [|] "IH'"; simpl.
-      { iMod "Hpost" as "Hpost". iModIntro. iNext.
-        do 2 (iMod "Hpost" as "Hpost"; iModIntro).
-        iDestruct "Hpost" as "[$ He₂]".
-        iApply ("IH" with "He₂ Himp" ). }
-      iMod "Hpost" as "Hpost". iModIntro. iNext.
-      iMod "Hpost" as "Hpost". iClear "IH".
-      iMod ("IH'" with "Hpost Himp") as "IH".
-      do 2 iModIntro. iNext. iApply "IH".
-  Qed.
-  
-  Lemma ewpw_mono_os E ρ e Φ Φ' `{! OSRow ρ} :
-    EWPW e @ E <| ρ |> {{ Φ }} -∗
-    (∀ v : val, Φ v ={E}=∗ Φ' v) -∗ 
-    EWPW e @E <| ρ |> {{ Φ' }}. 
-  Proof.
-    iIntros "Hewp HΦ". rewrite /ewpw.
-    assert (OSRow (filter_os ρ)).
-    { by apply sem_row_filter_os. }
-    iApply (@ewp_mono_os _ (filter_os ρ) ρ e Φ Φ' H _ with "Hewp HΦ").
-  Qed.
-  
-  Lemma ewpw_mono E ρ e Φ Φ' :
-    EWPW e @E <| ρ |> {{ Φ }} -∗
-    □ (∀ v : val, Φ v ={E}=∗ Φ' v) -∗ 
-    EWPW e @E <| ρ |> {{ Φ' }}.
-  Proof.
-    iIntros "Hewp HΦ". rewrite /ewpw. 
-    iApply (ewp_pers_mono with "Hewp HΦ").
-  Qed.
+Lemma ewpw_bot_inv e E Φ :
+  EWPW e @ E {{ Φ }} -∗
+  EWP e @ E {{ v, Φ v }}.
+Proof. 
+  iIntros "Hewp".
+  rewrite /ewpw /=.
+  rewrite filter_os_nil.
+  iApply ewp_ms_prot_mono.
+  { iApply row_nil_iEff_bot. }
+  iApply ewp_os_prot_mono.
+  { iApply row_nil_iEff_bot. }
+  iApply "Hewp".
+Qed.
 
-  Lemma ewpw_pure_step' E e e' ρ Φ :
-    pure_prim_step e e' → 
-    ▷ EWPW e' @E <| ρ |>  {{ Φ }} -∗
-    EWPW e @E <| ρ |> {{ Φ }}. 
-  Proof.
-    iIntros "%Hprim Hewp". rewrite /ewpw. 
-    by iApply ewp_pure_step'.
-  Qed.
-  
-  Lemma ewpw_bind k `{NeutralEctx k} E ρ e e' Φ  :
-    e' = fill k e →
-    EWPW e @E <| ρ |> {{ w, EWPW (fill k w) @E <| ρ |> {{ Φ }} }} -∗
-    EWPW e' @E <| ρ |> {{ Φ }}.
-  Proof.
-    iIntros (?) "Hewp". rewrite /ewpw. 
-    by iApply ewp_bind.
-  Qed.
-  
-  Lemma ewpw_alloc E ρ Φ v :
-    ▷ (∀ (l : loc), l ↦ v ={E}=∗ Φ #l) -∗
-      EWPW (ref v)%E @E <| ρ |> {{ Φ }}.
-  Proof.
-    iIntros "H". rewrite /ewpw. by iApply ewp_alloc. 
-  Qed.
-  
-  Lemma ewpw_load E ρ Φ l q v :
-    ▷ l ↦{q} v -∗
-      ▷ (l ↦{q} v ={E}=∗ Φ v) -∗
-        EWPW (Load #l)%E @E <| ρ |> {{ Φ }}.
-  Proof.
-    iIntros "H". rewrite /ewpw. by iApply ewp_load. 
-  Qed.
-  
-  Lemma ewpw_store E ρ Φ l v w :
-    ▷ l ↦ v -∗
-      ▷ (l ↦ w ={E}=∗ Φ #()) -∗
-        EWPW (#l <- w)%E @E <| ρ |> {{ Φ }}.
-  Proof.
-    iIntros "H". rewrite /ewpw. by iApply ewp_store. 
-  Qed.
-  
-  Lemma ewpw_replace E ρ Φ l v w :
-    ▷ l ↦ v -∗
-      ▷ (l ↦ w ={E}=∗ Φ v) -∗
-        EWPW (#l <!- w)%E @E <| ρ |> {{ Φ }}.
-  Proof.
-    iIntros "H". rewrite /ewpw. by iApply ewp_replace. 
-  Qed.
-  
-  Lemma ewpw_free E ρ Φ l v :
-    ▷ l ↦ v -∗
-      ▷ (|={E}=> Φ v) -∗
-        EWPW (Free #l)%E @E <| ρ |> {{ Φ }}.
-  Proof.
-    iIntros "H". rewrite /ewpw. by iApply ewp_free. 
-  Qed.
-  
-  Lemma ewpw_atomic E1 E2 e ρ Φ `{!Atomic StronglyAtomic e} :
-    TCEq (to_eff e) None →
-      (|={E1,E2}=> EWPW e @E2 <| ρ |> {{ v, |={E2,E1}=> Φ v }}) -∗
-        EWPW e @E1 <| ρ |> {{ Φ }}.
-  Proof.
-    iIntros (?) "H". rewrite /ewpw. by iApply ewp_atomic. 
-  Qed.
+Lemma ewpw_sub E e ρ ρ' Φ :
+  ρ ≤R ρ' -∗ 
+  EWPW e @E <| ρ |> {{ Φ }} -∗ EWPW e @E <| ρ' |> {{ Φ }}. 
+Proof.
+  iIntros "#Hρρ' Hewp".
+  rewrite /ewpw.
+  iApply ewp_ms_prot_mono; first (iApply (row_le_iEff with "Hρρ'")). 
+  iApply ewp_os_prot_mono; last done. 
+  { iApply row_le_iEff. by iApply row_le_filter_os_mono. }
+Qed.
 
-  Lemma ewpw_eff_os E ρ Φ v k :
-    iEff_car (upcl OS ⟦ filter_os ρ ⟧%R) v (λ w, ▷ EWPW (fill k (Val w)) @ E <| ρ |> {{ Φ }}) -∗
-    EWPW (of_eff OS v k) @ E <| ρ |> {{ Φ }}.
-  Proof. 
-    iIntros "H". rewrite /ewpw /=.
-    by iApply ewp_eff_os.
-  Qed.
+Lemma ewp_mono_os E (ρ ρ' : sem_row Σ) e Φ Φ' `{! OSRow ρ } `{! OSRow ρ' } :
+  EWP e @ E <| ⟦ ρ ⟧%R |> {| ⟦ ρ' ⟧%R |} {{ v, Φ v }} -∗
+  (∀ v : val, Φ v ={E}=∗ Φ' v) -∗ EWP e @ E <| ⟦ ρ ⟧%R |> {| ⟦ ρ' ⟧%R |} {{ v, Φ' v }}.
+Proof.
+  iIntros "Hewp Himp". 
+  iLöb as "IH" forall (e).
+  rewrite !ewp_unfold /ewp_pre.
+  destruct (to_val e) eqn:?.
+  { iMod "Hewp" as "Hewp". by iApply "Himp". }
+  destruct (to_eff e) eqn:?.
+  - simpl. destruct p eqn:?, p0 eqn:?, m;
+    iDestruct "Hewp" as "(%Φ'' & HΨ & Hps)";
+    iExists (λ w, Φ'' w ∗ (∀ v, Φ v ={E}=∗ Φ' v)%I)%I;
+    iSplitL "HΨ Himp".
+    2, 4: try (iDestruct "Hps" as "#Hps"; iModIntro);
+          iIntros "% (HΦ'' & Himp)"; 
+          iSpecialize ("Hps" with "HΦ''"); iNext;
+          iApply ("IH" with "Hps Himp").
+    + destruct OSRow0 as [];
+      iApply (monotonic_prot with "[Himp] HΨ"); iIntros "% $ {$Himp}".
+    + destruct OSRow1 as [];
+      iApply (monotonic_prot with "[Himp] HΨ"); iIntros "% $ {$Himp}".
+  - iIntros (σ₁ ns κ' κs nt) "Hstate".
+    iSpecialize ("Hewp" $! σ₁ ns κ' κs nt with "Hstate"). 
+    iMod "Hewp" as "Hewp". iModIntro.
+    iDestruct "Hewp" as "(Hred & Hpost)".
+    iFrame. iIntros (e₂ σ₂) "Hprim Hcred".
+    iSpecialize ("Hpost" $! e₂ σ₂ with "Hprim Hcred").
+    iInduction (num_laters_per_step) as [|] "IH'"; simpl.
+    { iMod "Hpost" as "Hpost". iModIntro. iNext.
+      do 2 (iMod "Hpost" as "Hpost"; iModIntro).
+      iDestruct "Hpost" as "[$ He₂]".
+      iApply ("IH" with "He₂ Himp" ). }
+    iMod "Hpost" as "Hpost". iModIntro. iNext.
+    iMod "Hpost" as "Hpost". iClear "IH".
+    iMod ("IH'" with "Hpost Himp") as "IH".
+    do 2 iModIntro. iNext. iApply "IH".
+Qed.
 
-  Lemma ewpw_do_os E l s v ρ Φ :
-    iEff_car ⟦ filter_os ρ ⟧%R ((effect l, s), v)%V Φ -∗ 
-    EWPW (do: ((effect l, s), v)%V) @ E <| ρ |> {{ Φ }}.
-  Proof.
-    iIntros "Hρ".
-    rewrite /ewpw /=. iApply ewp_do_os.
-    simpl. iExists Φ. iFrame. iIntros (w) "$".
-  Qed.
+Lemma ewpw_mono_os E ρ e Φ Φ' `{! OSRow ρ} :
+  EWPW e @ E <| ρ |> {{ Φ }} -∗
+  (∀ v : val, Φ v ={E}=∗ Φ' v) -∗ 
+  EWPW e @E <| ρ |> {{ Φ' }}. 
+Proof.
+  iIntros "Hewp HΦ". rewrite /ewpw.
+  assert (OSRow (filter_os ρ)).
+  { by apply row_filter_os_os_row. }
+  iApply (@ewp_mono_os _ (filter_os ρ) ρ e Φ Φ' H _ with "Hewp HΦ").
+Qed.
 
-  Lemma ewpw_do_ms E l s v ρ Φ :
-    iEff_car ⟦ ρ ⟧%R ((effect l, s), v)%V Φ -∗ 
-    EWPW (doₘ: ((effect l, s), v)%V) @ E <| ρ |> {{ Φ }}.
-  Proof.
-    iIntros "Hρ".
-    rewrite /ewpw /=. 
-    iApply ewp_do_ms;
-    simpl; iExists Φ; iFrame; iIntros "!# % $".
-  Qed.
+Lemma ewpw_mono E ρ e Φ Φ' :
+  EWPW e @E <| ρ |> {{ Φ }} -∗
+  □ (∀ v : val, Φ v ={E}=∗ Φ' v) -∗ 
+  EWPW e @E <| ρ |> {{ Φ' }}.
+Proof.
+  iIntros "Hewp HΦ". rewrite /ewpw. 
+  iApply (ewp_pers_mono with "Hewp HΦ").
+Qed.
 
-  Definition shallow_handler_wrp
+Lemma ewpw_pure_step' E e e' ρ Φ :
+  pure_prim_step e e' → 
+  ▷ EWPW e' @E <| ρ |>  {{ Φ }} -∗
+  EWPW e @E <| ρ |> {{ Φ }}. 
+Proof.
+  iIntros "%Hprim Hewp". rewrite /ewpw. 
+  by iApply ewp_pure_step'.
+Qed.
+
+Lemma ewpw_bind k `{NeutralEctx k} E ρ e e' Φ :
+  e' = fill k e →
+  EWPW e @E <| ρ |> {{ w, EWPW (fill k w) @E <| ρ |> {{ Φ }} }} -∗
+  EWPW e' @E <| ρ |> {{ Φ }}.
+Proof.
+  iIntros (?) "Hewp". rewrite /ewpw.
+  by iApply ewp_bind.
+Qed.
+
+Lemma ewpw_alloc E ρ Φ v :
+  ▷ (∀ (l : loc), l ↦ v ={E}=∗ Φ #l) -∗
+    EWPW (ref v)%E @E <| ρ |> {{ Φ }}.
+Proof.
+  iIntros "H". rewrite /ewpw. by iApply ewp_alloc. 
+Qed.
+
+Lemma ewpw_load E ρ Φ l q v :
+  ▷ l ↦{q} v -∗
+    ▷ (l ↦{q} v ={E}=∗ Φ v) -∗
+      EWPW (Load #l)%E @E <| ρ |> {{ Φ }}.
+Proof.
+  iIntros "H". rewrite /ewpw. by iApply ewp_load. 
+Qed.
+
+Lemma ewpw_store E ρ Φ l v w :
+  ▷ l ↦ v -∗
+    ▷ (l ↦ w ={E}=∗ Φ #()) -∗
+      EWPW (#l <- w)%E @E <| ρ |> {{ Φ }}.
+Proof.
+  iIntros "H". rewrite /ewpw. by iApply ewp_store. 
+Qed.
+
+Lemma ewpw_replace E ρ Φ l v w :
+  ▷ l ↦ v -∗
+    ▷ (l ↦ w ={E}=∗ Φ v) -∗
+      EWPW (#l <!- w)%E @E <| ρ |> {{ Φ }}.
+Proof.
+  iIntros "H". rewrite /ewpw. by iApply ewp_replace. 
+Qed.
+
+Lemma ewpw_free E ρ Φ l v :
+  ▷ l ↦ v -∗
+    ▷ (|={E}=> Φ v) -∗
+      EWPW (Free #l)%E @E <| ρ |> {{ Φ }}.
+Proof.
+  iIntros "H". rewrite /ewpw. by iApply ewp_free. 
+Qed.
+
+Lemma ewpw_atomic E1 E2 e ρ Φ `{!Atomic StronglyAtomic e} :
+  TCEq (to_eff e) None →
+    (|={E1,E2}=> EWPW e @E2 <| ρ |> {{ v, |={E2,E1}=> Φ v }}) -∗
+      EWPW e @E1 <| ρ |> {{ Φ }}.
+Proof.
+  iIntros (?) "H". rewrite /ewpw. by iApply ewp_atomic. 
+Qed.
+
+Lemma ewpw_eff_os E ρ Φ v k :
+  iEff_car (upcl OS ⟦ filter_os ρ ⟧%R) v (λ w, ▷ EWPW (fill k (Val w)) @ E <| ρ |> {{ Φ }}) -∗
+  EWPW (of_eff OS v k) @ E <| ρ |> {{ Φ }}.
+Proof. 
+  iIntros "H". rewrite /ewpw /=.
+  by iApply ewp_eff_os.
+Qed.
+
+Lemma ewpw_do_os E l s v ρ Φ :
+  iEff_car ⟦ filter_os ρ ⟧%R ((effect l, s), v)%V Φ -∗ 
+  EWPW (do: ((effect l, s), v)%V) @ E <| ρ |> {{ Φ }}.
+Proof.
+  iIntros "Hρ".
+  rewrite /ewpw /=. iApply ewp_do_os.
+  simpl. iExists Φ. iFrame. iIntros (w) "$".
+Qed.
+
+Lemma ewpw_do_ms E l s v ρ Φ :
+  iEff_car ⟦ ρ ⟧%R ((effect l, s), v)%V Φ -∗ 
+  EWPW (doₘ: ((effect l, s), v)%V) @ E <| ρ |> {{ Φ }}.
+Proof.
+  iIntros "Hρ".
+  rewrite /ewpw /=. 
+  iApply ewp_do_ms;
+  simpl; iExists Φ; iFrame; iIntros "!# % $".
+Qed.
+
+Lemma ewpw_lft l ρ e Φ :
+  EWPW e <| ρ |> {{ Φ }} -∗
+  EWPW (lft: (effect l, e)) <| ⦗ ρ | l ⦘ |> {{ Φ }}.
+Proof. 
+  iIntros "He".
+  rewrite /lft_def. rewrite /ewpw. ewp_pure_steps.
+  iApply (ewp_deep_try_with_mode with "[He]").
+  { ewp_pure_steps. iApply "He". }
+  iLöb as "IH".
+  rewrite {2} deep_handler_mode_unfold /deep_handler_mode_pre. 
+  iSplit; last iSplit.
+  - iIntros (v) "HΦ". by ewp_pure_steps.
+  - iIntros (v k) "Hρ".
+    iDestruct "Hρ" as "(%Φ' & (%w & %l' & %s' & %σ' & -> & #Hlookup' & Hσ') & HPost)". 
+    ewp_pure_steps'.
+    destruct (decide (l = l')) as [->|Hneg].
+    + ewp_pure_steps'. iApply ewp_do_os. 
+      rewrite filter_os_lookup. iExists Φ'. simpl.
+      iSplitL "Hσ'".
+      { iExists w, l', (S s'), σ'. rewrite filter_os_lookup row_tun_lookup_alt. iFrame "#∗". 
+        by replace (Z.add (Z.of_nat s') (Zpos xH)) with (Z.of_nat (S s')) by lia. }
+      iIntros (v') "HΦ'". iApply ("HPost" with "HΦ'"). by iNext.
+    + ewp_pure_steps'. iApply ewp_do_os. 
+      rewrite filter_os_lookup. iExists Φ'. simpl.
+      iSplitL "Hσ'".
+      { iExists w, l', s', σ'. rewrite filter_os_lookup row_tun_lookup_ne //. by iFrame "#∗".  }
+      iIntros (v') "HΦ'". iApply ("HPost" with "HΦ'"). by iNext.
+  - iIntros (v k) "Hρ". simpl.
+    iDestruct "Hρ" as "(%Φ' & (%w & %l' & %s' & %σ' & -> & #Hlookup' & Hσ') & #HPost)". 
+    ewp_pure_steps'.
+    destruct (decide (l = l')) as [->|Hneg].
+    + ewp_pure_steps'. iApply ewp_do_ms. 
+      iExists Φ'. simpl.
+      iSplitL "Hσ'".
+      { iExists w, l', (S s'), σ'. rewrite row_tun_lookup_alt. iFrame "#∗". 
+        by replace (Z.add (Z.of_nat s') (Zpos xH)) with (Z.of_nat (S s')) by lia. }
+      iIntros "!# %v' HΦ'". iApply ("HPost" with "HΦ'"). by iNext.
+    + ewp_pure_steps'. iApply ewp_do_ms. iExists Φ'. simpl.
+      iSplitL "Hσ'".
+      { iExists w, l', s', σ'. rewrite row_tun_lookup_ne //. by iFrame "#∗".  }
+      iIntros "!# %v' HΦ'". iApply ("HPost" with "HΦ'"). by iNext.
+Qed.
+
+Lemma ewpw_unlft l ρ e Φ :
+  EWPW e <| ⦗ ρ | l ⦘ |> {{ Φ }} -∗
+  EWPW (unlft: (effect l, e)) <| ρ |> {{ Φ }}.
+Proof.
+  iIntros "He".
+  rewrite /unlft_def. rewrite /ewpw. ewp_pure_steps.
+  iApply (ewp_deep_try_with_mode with "[He]").
+  { ewp_pure_steps. iApply "He". }
+  iLöb as "IH".
+  rewrite {2} deep_handler_mode_unfold /deep_handler_mode_pre. 
+  iSplit; last iSplit.
+  - iIntros (v) "HΦ". by ewp_pure_steps.
+  - iIntros (v k) "Hρ".
+    iDestruct "Hρ" as "(%Φ' & (%w & %l' & %s' & %σ' & -> & #Hlookup' & Hσ') & HPost)". 
+    ewp_pure_steps'.
+    destruct (decide (l = l')) as [->|Hneg].
+    + ewp_pure_steps'. iApply ewp_do_os. 
+      rewrite filter_os_lookup row_tun_lookup. 
+      iDestruct "Hlookup'" as "[(%s & -> & Hlookup) HOS]". iExists Φ'. simpl.
+      iSplitL "Hσ'".
+      { iExists w, l', s, σ'. rewrite filter_os_lookup. iFrame "#∗". 
+        by replace (Z.sub (Z.of_nat (S s)) (Zpos xH)) with (Z.of_nat s) by lia. }
+      iIntros (v') "HΦ'". iApply ("HPost" with "HΦ'"). by iNext.
+    + ewp_pure_steps'. iApply ewp_do_os. 
+      rewrite filter_os_lookup row_tun_lookup_ne //. iExists Φ'. simpl.
+      iSplitL "Hσ'".
+      { iExists w, l', s', σ'. rewrite filter_os_lookup //. by iFrame "#∗".  }
+      iIntros (v') "HΦ'". iApply ("HPost" with "HΦ'"). by iNext.
+  - iIntros (v k) "Hρ". simpl.
+    iDestruct "Hρ" as "(%Φ' & (%w & %l' & %s' & %σ' & -> & #Hlookup' & Hσ') & #HPost)". 
+    ewp_pure_steps'.
+    destruct (decide (l = l')) as [->|Hneg].
+    + ewp_pure_steps'. iApply ewp_do_ms. 
+      rewrite row_tun_lookup. iDestruct "Hlookup'" as "(%s & -> & Hlookup)". 
+      iExists Φ'. simpl.
+      iSplitL "Hσ'".
+      { iExists w, l', s, σ'. iFrame "#∗". 
+        by replace (Z.sub (Z.of_nat (S s)) (Zpos xH)) with (Z.of_nat s) by lia. }
+      iIntros "!# %v' HΦ'". iApply ("HPost" with "HΦ'"). by iNext.
+    + ewp_pure_steps'. iApply ewp_do_ms. iExists Φ'. simpl.
+      iSplitL "Hσ'".
+      { iExists w, l', s', σ'. rewrite row_tun_lookup_ne //. by iFrame "#∗".  }
+      iIntros "!# %v' HΦ'". iApply ("HPost" with "HΦ'"). by iNext.
+Qed.
+
+Lemma handler_effect_propagated_cond E l l' s' Ψ :
+ ¬ (l = l' ∧ s' = 0) →
+ ⊢ EWP if: (effect l')%V = (effect l)%V then #s' = #0 else #false @ E <| Ψ |> {{ v, ⌜v = #false⌝ }}.
+Proof.
+  intros Hneg. rewrite not_and_l in Hneg. iIntros.
+  destruct (decide (l = l')) as [->|], Hneg; ewp_pure_steps'. 
+  iPureIntro. rewrite bool_decide_false //. 
+  intros H'. simplify_eq. assert (s' = 0) by lia. simplify_eq. 
+Qed.
+
+Definition shallow_handler_ls
   (E : coPset)
+  (l : label)
+  (σ : sem_sig Σ)
   (ρ : sem_row Σ)
-  (Φ : val -d> iProp Σ)
+  (m : mode)
+  (Φ : val -d> iPropO Σ)
   (h r : expr)
-  (ρ' : sem_row Σ)
-  (Φ' : val -d> iProp Σ) : iProp Σ :=
-    shallow_handler E ⟦ filter_os ρ ⟧%R ⟦ ρ ⟧%R Φ h r
-                      ⟦ filter_os ρ' ⟧%R ⟦ ρ' ⟧%R Φ'.
+  (ρ'  : sem_row Σ)
+  (Φ' : val -d> iPropO Σ) : iProp Σ := (
+  (* Subsumption on row *)
+  (ρ ≤R ρ') ∗
 
-  
-  Definition shallow_handler_wrp_os
-    (E : coPset)
-    (ρ : sem_row Σ)
-    (Φ : val -d> iPropO Σ)
-    (h r : expr)
-    (ρ' : sem_row Σ)
-    (Φ' : val -d> iPropO Σ) : iProp Σ :=
+  (* One-Shot Row *)
+  (⌜ m = OS → OSRow ρ ⌝) ∗
 
-    (* Correctness of the return branch. *)
-    (∀ (y : val), Φ y -∗ EWPW r y @ E <| ρ' |> {{ Φ' }}) ∧
+  □?m (
+  (* Correctness of the return branch. *)
+  (∀ (v : val), Φ v -∗ EWPW r v @ E <| ρ' |> {{ Φ' }}) ∧
 
-    (* Correctness of the effect branch. *)
-    (∀ (v k : val),
-       iEff_car (upcl OS ⟦ ρ ⟧%R) v (λ w, EWPW k w @ E <| ρ |> {{ Φ }}) -∗
-         EWPW h v k @ E <| ρ' |> {{ Φ' }}).
+  (* Correctness of the effect branch. *)
+  (∀ (v k : val),
+     iEff_car (upcl σ.1 σ.2) v (λ w, EWPW k w @ E <| (l, σ) · ρ |> {{ Φ }}) -∗
+       EWPW h v k @ E <| ρ' |> {{ Φ' }}))
+  )%I.
 
-  Lemma iEff_le_upcl_ms_os (Ψ : iEff Σ) :
-    ⊢ iEff_le (upcl MS Ψ) (upcl OS Ψ).
-  Proof.
-    iIntros (v Φ) "!# HMSΨ". rewrite /upcl /=.
-    iDestruct "HMSΨ" as "(%Φ' & HΨΦ' & #HPost)".
-    iExists Φ'. iFrame "#∗".
-  Qed.
-  
-  Lemma shallow_handler_wrp_os_impl E ρ Φ h r ρ' Φ' :
-    shallow_handler_wrp_os E ρ Φ h r ρ' Φ' -∗
-    shallow_handler_wrp E ρ Φ h r ρ' Φ'.
-  Proof.
-    iIntros "H". rewrite /shallow_handler_wrp_os /shallow_handler_wrp /ewpw.
-    rewrite /shallow_handler. repeat iSplit.
-    - iDestruct "H" as "[H _]". iApply "H".
-    - iDestruct "H" as "[_ H]"; iIntros (v k) "Hρ"; iApply "H". 
-      iApply iEff_le_upcl; last done.
-      iApply row_le_iEff. iApply row_le_filter_os_elim.
-    - iDestruct "H" as "[_ H]"; iIntros (v k) "Hρ"; iApply "H".
-      by iApply iEff_le_upcl_ms_os.
-  Qed.
+Lemma ewpw_shallow_try_ls E (l : label) m σ ρ ρ' e (h r : val) Φ Φ' :
+  EWPW e @ E <| (l, σ) · ρ |> {{ Φ }} -∗
+  shallow_handler_ls E l σ ρ m Φ h r ρ' Φ' -∗
+  EWPW (ShallowTryLSV e l h r) @E <| ρ' |> {{ Φ' }}.
+Proof.
+  iIntros "He H". rewrite /ShallowTryLSV /shallow_try_ls /ewpw. 
+  iLöb as "IH" forall (e). ewp_pure_steps.
+  iApply (ewp_try_with_mode with "He").
+  rewrite /shallow_handler_ls.
+  iDestruct "H" as "(#Hle & %HOS & Hbr)". 
+  iSplit; last iSplit.
+  - rewrite {2} bi.intuitionistically_if_elim. iDestruct "Hbr" as "[$ _]".
+  - iIntros (v k) "Hρ".
+    ewp_pure_steps. 
+    iDestruct "Hρ" as "(%Φ'' & (%v' & %l' & %s' & %σ' & %Heq' & Hlookup' & Hσ') & HPost)".
+    inv Heq'. destruct (decide (l = l' ∧ s' = 0)) as [[-> ->]|Hneg].
+    + ewp_pure_steps'.
+      rewrite {2} bi.intuitionistically_if_elim. iDestruct "Hbr" as "[_ H]".
+      iApply "H". iExists Φ''. 
+      rewrite filter_os_lookup lookup_insert.
+      iDestruct "Hlookup'" as "[#Heq #HσOS]".
+      rewrite option_equivI. iRewrite - "Heq" in "HσOS".
+      rewrite prod_equivI_2 (iEff_equivI σ.2 σ'.2).
+      iRewrite - ("Heq" $! v' Φ'') in "Hσ'". iFrame. 
+      iRewrite "HσOS". simpl. iIntros (w) "Φ''". by iApply "HPost".
+    + do 19 ewp_value_or_step. iApply (ewp_if_false with "[]").
+      { by iApply handler_effect_propagated_cond. }
+      ewp_pure_steps.
+      iApply ewp_do_os. iExists Φ''. simpl. 
+      iPoseProof (row_le_filter_os_mono with "Hle") as "Hlef".
+      rewrite filter_os_lookup lookup_insert_ne; last (intros H'; inv H'; tauto).
+      rewrite - filter_os_lookup.
+      iDestruct ("Hlef" with "Hlookup'") as "(%σ'' & Hlookup'' & [Hmle'' Hle''])".
+      iSplitR "HPost Hbr".
+      { iExists v', l', s', σ''. iFrame "#∗". iSplit; first done. by iApply "Hle''". }
+      iIntros (w) "HΦ''". do 5 ewp_value_or_step.
+      iApply ("IH" with "[HΦ'' HPost] [Hbr]"); first by iApply "HPost".
+      by iFrame "#∗".
+  - iIntros (v k) "Hρ".
+    ewp_pure_steps. 
+    iDestruct "Hρ" as "(%Φ'' & (%v' & %l' & %s' & %σ' & %Heq' & #Hlookup' & Hσ') & #HPost)".
+    inv Heq'. destruct (decide (l = l' ∧ s' = 0)) as [[-> ->]|Hneg].
+    + ewp_pure_steps'.
+      rewrite {2} bi.intuitionistically_if_elim. iDestruct "Hbr" as "[_ H]".
+      iApply "H". iExists Φ''. 
+      rewrite lookup_insert option_equivI prod_equivI_2 iEff_equivI.
+      iRewrite - ("Hlookup'" $! v' Φ'') in "Hσ'". iFrame.
+      destruct σ.1; simpl; last iIntros "!#"; iIntros (w) "Φ''"; by iApply "HPost".
+    + do 19 ewp_value_or_step. iApply (ewp_if_false with "[]").
+      { by iApply handler_effect_propagated_cond. }
+      ewp_pure_steps. rewrite lookup_insert_ne; last (intros H'; inv H'; tauto).
+      iApply ewp_do_ms. destruct m; simpl.
+      * specialize (HOS eq_refl).
+        iDestruct (os_row_mono_prot ρ l' s' σ' with "Hlookup'") as "Hmono".
+        iAssert (shallow_handler_ls E l σ ρ OS Φ h r ρ' Φ') with "[Hbr]" as "H".
+        { rewrite /shallow_handler_ls. simpl. by iFrame "#∗". }
+        iExists (λ v, Φ'' v ∗ shallow_handler_ls E l σ ρ OS Φ h r ρ' Φ')%I.
+        iSplitL; [|iIntros "!# %w [HΦ'' H]"; do 5 ewp_value_or_step; 
+                   iSpecialize ("HPost" with "HΦ''"); iApply ("IH" with "HPost H")].
+        iDestruct ("Hle" with "Hlookup'") as "(%σ'' & Hlookup'' & [Hmle'' Hle''])".
+        iExists v', l', s', σ''. iFrame "#∗".
+        iSplit; [done|iApply "Hle''"]. iApply ("Hmono" with "[H] Hσ'"). iIntros (w) "$ //".
+      * iDestruct "Hbr" as "#Hbr".
+        iDestruct ("Hle" with "Hlookup'") as "(%σ'' & Hlookup'' & [Hmle'' Hle''])".
+        iExists Φ''. iSplitL "Hσ'".
+        { iExists v', l', s', σ''. iFrame "#∗". iSplit; first done. by iApply "Hle''". }
+        iIntros (w) "!# HΦ''". do 5 ewp_value_or_step.
+        iApply ("IH" with "[HΦ'' HPost] [Hbr]"); first by iApply "HPost".
+        by iFrame "#∗".
+Qed.
 
-  Lemma ewpw_try_with E ρ Φ ρ' Φ' e h r :
-    EWPW e @ E <| ρ |> {{ Φ }} -∗
-      shallow_handler_wrp E ρ Φ h r ρ' Φ' -∗
-        EWPW (TryWith e h r) @ E <| ρ' |> {{ Φ' }}.
-  Proof.
-    iIntros "Hewp H". rewrite /shallow_handler_wrp /ewpw. 
-    iApply (ewp_try_with with "Hewp"); iApply "H".
-  Qed.
+Notation deep_handler_ls_type Σ :=
+  (coPset -d> label-d> sem_sig Σ -d> sem_row Σ -d> mode -d> (val -d> iPropO Σ) 
+          -d> expr -d> expr
+          -d> sem_row Σ -d> (val -d> iPropO Σ) -d> iPropO Σ) (only parsing).
 
-  Definition deep_handler_wrp
-  (E : coPset)
-  (ρ : sem_row Σ)
-  (Φ : val -d> iProp Σ)
-  (h r : expr)
-  (ρ' : sem_row Σ)
-  (Φ' : val -d> iProp Σ) : iProp Σ :=
-    deep_handler E ⟦ filter_os ρ ⟧%R ⟦ ρ ⟧%R Φ h r
-                   ⟦ filter_os ρ' ⟧%R ⟦ ρ' ⟧%R Φ'.
+Definition deep_handler_ls_pre `{irisGS eff_lang Σ} : 
+  deep_handler_ls_type Σ → deep_handler_ls_type Σ := (
+  λ deep_handler_ls E l σ ρ m Φ h r ρ' Φ',
+  (* Subsumption on row *)
+  (ρ ≤R ρ') ∗
 
-  Definition deep_handler_wrp_os
-    (E : coPset)
-    (ρ : sem_row Σ)
-    (Φ : val -d> iPropO Σ)
-    (h r : expr)
-    (ρ' : sem_row Σ)
-    (Φ' : val -d> iPropO Σ) : iProp Σ :=
+  (* One-Shot Row *)
+  (⌜ m = OS → OSRow ρ ⌝) ∗
 
-    (* Correctness of the return branch. *)
-    (∀ (y : val), Φ y -∗ EWPW r y @ E <| ρ' |> {{ Φ' }}) ∧
+  □?m (
+  (* Correctness of the return branch. *)
+  (∀ (v : val), Φ v -∗ EWPW r v @ E <| ρ' |> {{ Φ' }}) ∧
 
-    (* Correctness of the effect branch. *)
-    (∀ (v k : val),
-       iEff_car (upcl OS ⟦ ρ ⟧%R) v (λ w, ∀ Ψ' Ψ'' Φ'',
-          ▷ deep_handler E ⟦ filter_os ρ ⟧%R ⟦ ρ ⟧%R Φ h r Ψ' Ψ'' Φ'' -∗
-          EWP k w @ E <| Ψ' |> {| Ψ'' |} {{ Φ'' }}) -∗
-         EWPW h v k @ E <| ρ' |> {{ Φ' }}).
+  (* Correctness of the effect branch. *)
+  (∀ (v k : val),
+     iEff_car (upcl σ.1 σ.2) v (λ w, 
+        ∀ ρ'' Φ'', 
+          ▷ deep_handler_ls E l σ ρ m Φ h r ρ'' Φ'' -∗
+          EWPW k w @ E <| ρ'' |> {{ Φ'' }}
+     ) -∗
+       EWPW h v k @ E <| ρ' |> {{ Φ' }}))
+  )%I.
 
-  Lemma deep_handler_wrp_os_impl E ρ Φ h r ρ' Φ' :
-    deep_handler_wrp_os E ρ Φ h r ρ' Φ' -∗
-    deep_handler_wrp E ρ Φ h r ρ' Φ'.
-  Proof.
-    iIntros "H". rewrite /deep_handler_wrp_os /deep_handler_wrp /ewpw.
-    rewrite deep_handler_unfold. repeat iSplit.
-    - iDestruct "H" as "[H _]"; iApply "H".
-    - iDestruct "H" as "[_ H]"; iIntros (v k) "Hρ".
-      iApply "H". iApply iEff_le_upcl; last done.
-      iApply row_le_iEff. iApply row_le_filter_os_elim.
-    - iDestruct "H" as "[_ H]". iIntros (v k) "H'".
-      iApply "H". by iApply iEff_le_upcl_ms_os. 
-  Qed.
+Local Instance deep_handler_ls_pre_contractive `{irisGS eff_lang Σ} : Contractive deep_handler_ls_pre.
+Proof.
+  rewrite /deep_handler_ls_pre => n deep deep' Hne E l σ ρ m Φ h r ρ' Φ'.
+  repeat (f_contractive || f_equiv). intros ?; simpl.
+  repeat (f_contractive || f_equiv); apply Hne.
+Qed.
+Definition deep_handler_ls `{irisGS eff_lang Σ} := fixpoint deep_handler_ls_pre.
+Arguments deep_handler_ls _ _%V _%S _%R _%I _%E _%E _%R _%I.
 
-  Lemma ewpw_deep_try_with E ρ Φ (h r : val) ρ' Φ' e :
-    EWPW e @ E <| ρ |> {{ Φ }} -∗
-      deep_handler_wrp E ρ Φ h r ρ' Φ' -∗
-        EWPW DeepTryWithV e h r @ E <| ρ' |> {{ Φ' }}.
-  Proof.
-    iIntros "Hewp H". rewrite /deep_handler_wrp /ewpw. 
-    iApply (ewp_deep_try_with with "Hewp"); iApply "H".
-  Qed.
+Global Lemma deep_handler_ls_unfold `{irisGS eff_lang Σ} E l σ ρ m Φ h r ρ' Φ' :
+  deep_handler_ls E l σ ρ m Φ h r ρ' Φ' ⊣⊢
+    deep_handler_ls_pre deep_handler_ls E l σ ρ m Φ h r ρ' Φ'.
+Proof.
+  by apply (fixpoint_unfold deep_handler_ls_pre).
+Qed.
+
+Lemma ewpw_deep_try_ls E (l : label) m σ ρ ρ' e (h r : val) Φ Φ' :
+  EWPW e @ E <| (l, σ) · ρ |> {{ Φ }} -∗
+  deep_handler_ls E l σ ρ m Φ h r ρ' Φ' -∗
+  EWPW (DeepTryLSV e l h r) @E <| ρ' |> {{ Φ' }}.
+Proof.
+  iIntros "He H". rewrite /DeepTryLSV /deep_try_ls /ewpw. 
+  ewp_pure_steps.
+  iApply (ewp_deep_try_with_mode with "He").
+  iLöb as "IH" forall (ρ' Φ'). rewrite deep_handler_ls_unfold.
+  iDestruct "H" as "(#Hle & %HOS & Hbr)". 
+  rewrite deep_handler_mode_unfold /deep_handler_mode_pre.
+  iSplit; last iSplit.
+  - rewrite bi.intuitionistically_if_elim. iDestruct "Hbr" as "[$ _]".
+  - iIntros (v k) "Hρ". ewp_pure_steps. 
+    iDestruct "Hρ" as "(%Φ'' & (%v' & %l' & %s' & %σ' & %Heq' & Hlookup' & Hσ') & HPost)".
+    inv Heq'. destruct (decide (l = l' ∧ s' = 0)) as [[-> ->]|Hneg].
+    + ewp_pure_steps'.
+      rewrite bi.intuitionistically_if_elim. iDestruct "Hbr" as "[_ H]".
+      iApply "H". iExists Φ''. 
+      rewrite filter_os_lookup lookup_insert.
+      iDestruct "Hlookup'" as "[#Heq #HσOS]".
+      rewrite option_equivI. iRewrite - "Heq" in "HσOS".
+      rewrite prod_equivI_2 (iEff_equivI σ.2 σ'.2).
+      iRewrite - ("Heq" $! v' Φ'') in "Hσ'". iFrame. 
+      iRewrite "HσOS". simpl. iIntros (w) "HΦ''". 
+      iIntros (ρ'' Φ''') "Hdeep". iApply ("HPost" with "HΦ''").
+      iNext. iApply ("IH" with "Hdeep"). 
+    + do 19 ewp_value_or_step.
+      iApply (ewp_if_false with "[]"); first by iApply handler_effect_propagated_cond.
+      ewp_pure_steps. iApply ewp_do_os. iExists Φ''. simpl. 
+      iPoseProof (row_le_filter_os_mono with "Hle") as "Hlef".
+      rewrite filter_os_lookup lookup_insert_ne; last (intros H'; inv H'; tauto).
+      rewrite - filter_os_lookup.
+      iDestruct ("Hlef" with "Hlookup'") as "(%σ'' & Hlookup'' & [Hmle'' Hle''])".
+      iSplitR "HPost Hbr".
+      { iExists v', l', s', σ''. iFrame "#∗". iSplit; first done. by iApply "Hle''". }
+      iIntros (w) "HΦ''". iApply ("HPost" with "HΦ''"). iNext. iApply ("IH" with "[Hbr]").
+      destruct m; rewrite deep_handler_ls_unfold /deep_handler_ls_pre; iFrame "#∗"; eauto.
+  - iIntros (v k) "Hρ". ewp_pure_steps. 
+    iDestruct "Hρ" as "(%Φ'' & (%v' & %l' & %s' & %σ' & %Heq' & #Hlookup' & Hσ') & #HPost)".
+    inv Heq'. destruct (decide (l = l' ∧ s' = 0)) as [[-> ->]|Hneg].
+    + ewp_pure_steps'.
+      rewrite bi.intuitionistically_if_elim. iDestruct "Hbr" as "[_ H]".
+      iApply "H". iExists Φ''. 
+      rewrite lookup_insert option_equivI prod_equivI_2 iEff_equivI.
+      iRewrite - ("Hlookup'" $! v' Φ'') in "Hσ'". iFrame.
+      destruct σ.1; simpl; last iIntros "!#"; 
+      iIntros (w) "HΦ'' % %Φ''' Hdeep"; iApply ("HPost" with "HΦ''"); iNext; by iApply "IH".
+    + do 19 ewp_value_or_step.
+      iApply (ewp_if_false with "[]"); first by iApply handler_effect_propagated_cond.
+      ewp_pure_steps. rewrite lookup_insert_ne; last (intros H'; inv H'; tauto).
+      iApply ewp_do_ms. destruct m; simpl.
+      * specialize (HOS eq_refl).
+        iDestruct (os_row_mono_prot ρ l' s' σ' with "Hlookup'") as "Hmono".
+        iAssert (deep_handler_ls E l σ ρ OS Φ h r ρ' Φ') with "[Hbr]" as "H".
+        { rewrite deep_handler_ls_unfold /deep_handler_ls_pre. simpl. by iFrame "#∗". }
+        iExists (λ v, Φ'' v ∗ deep_handler_ls E l σ ρ OS Φ h r ρ' Φ')%I.
+        iSplitL; [|iIntros "!# %w [HΦ'' Hdeep]"; iApply ("HPost" with "HΦ''"); iNext; by iApply "IH"].
+        iDestruct ("Hle" with "Hlookup'") as "(%σ'' & Hlookup'' & [Hmle'' Hle''])".
+        iExists v', l', s', σ''. iFrame "#∗".
+        iSplit; [done|iApply "Hle''"]. iApply ("Hmono" with "[H] Hσ'"). iIntros (w) "$ //".
+      * iDestruct "Hbr" as "#Hbr".
+        iDestruct ("Hle" with "Hlookup'") as "(%σ'' & Hlookup'' & [Hmle'' Hle''])".
+        iExists Φ''. iSplitL "Hσ'".
+        { iExists v', l', s', σ''. iFrame "#∗". iSplit; first done. by iApply "Hle''". }
+        iIntros (w) "!# HΦ''". iApply ("HPost" with "HΦ''").
+        iNext. iApply "IH".
+        rewrite deep_handler_ls_unfold /deep_handler_ls_pre. simpl. by iFrame "#∗". 
+Qed.
 
 End reasoning.
