theories/logic/sem_row.v
@@ -15,8 +15,6 @@ From hazel.program_logic Require Import weakest_precondition
 (* Local imports *)
 From haffel.lib Require Import logic.
 From haffel.lang Require Import haffel.
-From haffel.lang Require Import subst_map.
-From haffel.logic Require Import iEff.
 From haffel.logic Require Import sem_def.
 From haffel.logic Require Import mode.
 From haffel.logic Require Import sem_sig.
@@ -24,16 +22,16 @@ From haffel.logic Require Import sem_sig.
 Definition sem_row_nil {Σ} : sem_row Σ := ∅. 
 Global Instance sem_row_bottom {Σ} : Bottom (sem_row Σ) := sem_row_nil.
 
-Definition sem_row_ins {Σ} (l : string) (σ : sem_sig Σ) (ρ : sem_row Σ) : sem_row Σ := 
+Definition sem_row_ins {Σ} (l : label) (σ : sem_sig Σ) (ρ : sem_row Σ) : sem_row Σ := 
   insert (l, 0) σ ρ.
 
 Definition sem_row_os {Σ} (ρ : sem_row Σ) : sem_row Σ := 
   fmap (λ σ, (σ.1, upcl OS σ.2)) ρ. 
 
 Definition sem_row_tun_f l := 
-  (λ k : stringO * nat, if decide (l = k.1) then (k.1, S k.2)
+  (λ k : label * nat, if decide (l = k.1) then (k.1, S k.2)
                                             else (k.1, k.2)).
-Definition sem_row_tun {Σ} (l : string) (ρ : sem_row Σ) : sem_row Σ := 
+Definition sem_row_tun {Σ} (l : label) (ρ : sem_row Σ) : sem_row Σ := 
   kmap (sem_row_tun_f l) ρ. 
 
 Local Instance inj_sem_row_tun l : Inj eq eq (sem_row_tun_f l).
@@ -52,6 +50,22 @@ Next Obligation.
   intros ???????. by repeat f_equiv. 
 Qed.
 
+
+Definition filter_os {Σ} (ρ : gmap (label * nat) (sem_sig Σ)) : sem_row Σ :=
+  union_with (λ (σ : sem_sig Σ) _, match σ.1 with 
+                        OS => Some σ
+                     |  MS => None end) ρ ρ.
+
+(* Notations. *)
+
+Notation "⟨⟩" := (sem_row_nil) : sem_row_scope.
+Notation "lσ · ρ" := (sem_row_ins lσ.1%S lσ.2%S ρ%R) (at level 80, right associativity) : sem_row_scope.
+Notation "¡ ρ" := (sem_row_os ρ%R) (at level 10) : sem_row_scope.
+Notation "⦗ ρ | l ⦘" := (sem_row_tun l%string ρ%R) (at level 5) : sem_row_scope.
+Notation "⟦ ρ ⟧" := (sem_row_iEff ρ%R) : sem_row_scope.
+
+(*  Properties *)
+
 Global Instance sem_row_iEff_ne {Σ} :
   NonExpansive (@sem_row_iEff Σ).
 Proof.
@@ -63,12 +77,7 @@ Global Instance sem_row_iEff_proper {Σ} :
   Proper ((≡) ==> (≡)) (@sem_row_iEff Σ).
 Proof. apply ne_proper. apply _. Qed.
 
-Definition filter_os {Σ} (ρ : gmap (string * nat) (sem_sig Σ)) : sem_row Σ :=
-  union_with (λ (σ : sem_sig Σ) _, match σ.1 with 
-                        OS => Some σ
-                     |  MS => None end) ρ ρ.
-
-Instance filter_os_ne {Σ} :
+Global Instance filter_os_ne {Σ} :
   NonExpansive (@filter_os Σ).
 Proof.
   intros ????. rewrite /filter_os.
@@ -79,114 +88,20 @@ Proof.
   simpl in *; by subst.
 Qed.
 
-Instance filter_os_proper {Σ} :
+Global Instance filter_os_proper {Σ} :
   Proper ((≡) ==> (≡)) (@filter_os Σ).
 Proof. apply ne_proper. apply _. Qed.
 
-
-(* Notations. *)
-
-Notation "⟨⟩" := (sem_row_nil) : sem_row_scope.
-Notation "lσ · ρ" := (sem_row_ins lσ.1%S lσ.2%S ρ%R) (at level 80, right associativity) : sem_row_scope.
-Notation "¡ ρ" := (sem_row_os ρ%R) (at level 10) : sem_row_scope.
-Notation "⦗ ρ | l ⦘" := (sem_row_tun l%string ρ%R) (at level 5) : sem_row_scope.
-Notation "⟦ ρ ⟧" := (sem_row_iEff ρ%R) : sem_row_scope.
-
-(* One-Shot Rows *)
-
-Notation OSRow ρ := (MonoProt ⟦ ρ%R ⟧)%R.
-
-Global Instance sem_row_nil_os_row {Σ} :
-  OSRow (⟨⟩ : sem_row Σ).
+Lemma filter_os_nil {Σ} :
+  filter_os (⟨⟩ : sem_row Σ)%R = (⟨⟩ : sem_row Σ)%R.
 Proof.
-  constructor. rewrite /sem_row_iEff /= /sem_row_nil.
-  iIntros (v Φ Φ') "_ (% & % & % & % & _ & H & _)".
-  rewrite lookup_empty. iDestruct "H" as "%". inv H. 
-Qed.
-  
-(* TODO: This needs to be generalised, 
-         if (l, 0) ∈ ρ then ρ(l, 0) does not need to be an OSSig.
-   NOTE: we can have a separate gset of keys that we don't need to check,
-         by creating a helper class *)
-Global Instance sem_row_ins_os_row {Σ} (ρ : sem_row Σ) l σ `{ OSSig σ, OSRow ρ } :
-  OSRow ((l, σ) · ρ).
-Proof.
-  constructor. iIntros (v Φ Φ') "HPost".
-  rewrite /sem_row_iEff /=.
-  iIntros "(%w & %l' & %s' & %σ' & -> & #Hlookup' & Hσ')".
-  destruct (decide ((l, 0) = (l', s'))). 
-  - rewrite /sem_row_ins. inv e. 
-    iExists w, l', 0, σ'. rewrite lookup_insert. 
-    iSplitR; first done. iFrame "#". 
-    iDestruct (option_equivI with "Hlookup'") as "#Hlookup''".
-    inv OSSig0. 
-    iDestruct (monotonic_prot w Φ Φ' with "HPost") as "H".
-    iDestruct (iEff_equivI σ.2 σ'.2) as "[Heq _]".
-    iSpecialize ("Heq" with "[]"); first by iRewrite "Hlookup''".
-    iRewrite ("Heq" $! w Φ) in "H". 
-    iRewrite ("Heq" $! w Φ') in "H". 
-    by iApply "H".
-  - inv OSRow0. rewrite /sem_row_iEff /= in monotonic_prot.
-    iDestruct (monotonic_prot (#(LitStr l'), #s', w)%V Φ Φ' with "HPost [Hσ']") as "(%w'' & %l'' & %s'' & %σ'' & %Heq & Hlookup & Hieff)".
-    { iExists w, l', s', σ'. iSplit; first done.
-      rewrite lookup_insert_ne; last done. iFrame "∗#". }
-    inv Heq. iExists w'', l'', s'', σ''. iSplitR; first done.
-    rewrite /sem_row_ins lookup_insert_ne; last done. iFrame "∗".
+  rewrite /filter_os.
+  rewrite union_with_idemp; first done.
+  intros ?? H. rewrite lookup_empty in H. inv H.
 Qed.
 
-Global Instance sem_row_tun_os_row {Σ} (l : string) (ρ : sem_row Σ) `{ OSRow ρ } :
-  OSRow ⦗ ρ | l ⦘.
-Proof.
-  constructor. rewrite /sem_row_iEff /=. 
-  iIntros (v Φ Φ') "HPost".
-  iIntros "(%v' & %l' & %s' & %σ' & #Heq & #Hlookup & Hσ)".
-  destruct (decide (l = l')) as [->|Hll']; first destruct s'.
-  - destruct (lookup_kmap_None (sem_row_tun_f l') ρ (l', 0)) as [_ H].
-    rewrite H; first (iDestruct "Hlookup" as "%H'"; inv H').
-    intros [l'' s''] H'. rewrite /sem_row_tun_f /= in H'.
-    destruct (decide (l' = l'')) eqn:H''. rewrite H'' in H'; first inv H'.
-    rewrite decide_False in H'; last done. inv H'.
-  - replace (l', S s') with (sem_row_tun_f l' (l', s')); last rewrite /sem_row_tun_f /= decide_True //.
-    rewrite lookup_kmap. inv OSRow0.
-    iDestruct (monotonic_prot (effect l', #s', v')%V Φ Φ' with "HPost [Hσ]") as "(%w & %l'' & %s'' & %σ'' & Heq' & Hlookup'' & Hσ'')".
-    { iExists v', l', s', σ'. by iFrame "#∗". }
-    iExists v', l', (S s'), σ''. iDestruct "Heq'" as "%". inv H.
-    iFrame "#∗".
-    replace (l'', S s'') with (sem_row_tun_f l'' (l'', s'')); last rewrite /sem_row_tun_f /= decide_True //.
-    rewrite lookup_kmap //.
-  - replace (l', s') with (sem_row_tun_f l (l', s')); last rewrite /sem_row_tun_f /= decide_False //. 
-    rewrite lookup_kmap. inv OSRow0.
-    rewrite /sem_row_iEff /= in monotonic_prot.
-    iDestruct (monotonic_prot (effect l', #s', v')%V Φ Φ' with "HPost [Hσ]") as "(%w & %l'' & %s'' & %σ'' & Heq' & Hlookup' & Hσ')".
-    { iExists v', l', s', σ'. by iFrame "#∗". }
-    iExists v', l', s', σ''. iDestruct "Heq'" as "%". inv H.
-    iRewrite "Heq"; iSplitR; first done. iFrame.
-    assert (H : (l'', s'') = sem_row_tun_f l (l'', s'')). 
-    { rewrite /sem_row_tun_f /= decide_False //. }
-    rewrite {3} H. rewrite /sem_row_tun lookup_kmap //. 
-Qed.
-
-Global Instance sem_row_os_os_row {Σ} (ρ : sem_row Σ) :
-  OSRow (¡ ρ ).
-Proof.
-  constructor. rewrite /sem_row_iEff /=.
-  iIntros (v Φ Φ') "HPost (% & % & % & % & Heq & #Hlookup & Hσ)".
-  iExists v', l, s, σ. iFrame "∗#".
-  rewrite /sem_row_os lookup_fmap.
-  destruct (ρ !! (l, s)) eqn:H; rewrite H /=. 
-  - iDestruct (option_equivI with "Hlookup") as "#Hlookup'".
-    destruct σ. simpl.
-    iDestruct (prod_equivI with "Hlookup'") as "[_ Heq]". simpl.
-    iDestruct (iEff_equivI (upcl OS o.2) o1) as "[Heq' _]".
-    iSpecialize ("Heq'" with "Heq"). iRewrite - ("Heq'" $! v' Φ').
-    pose proof (upcl_mono_prot o.2) as [].
-    iApply (monotonic_prot with "HPost").
-    by iRewrite ("Heq'" $! v' Φ).
-  - iDestruct "Hlookup" as "%H'". inv H'.
-Qed.
-
-Lemma filter_os_lookup {Σ} (ρ : sem_row Σ) (l : string) (s : nat) (σ : sem_sig Σ) :
-  (filter_os ρ !! (l, s) ≡ Some σ : iProp Σ) ∗-∗
+Lemma filter_os_lookup {Σ} (ρ : sem_row Σ) (l : label) (s : nat) (σ : sem_sig Σ) :
+  (filter_os ρ !! (l, s) ≡ Some σ : iProp Σ) ⊣⊢
   (ρ !! (l, s) ≡ Some σ ∗ σ.1 ≡ OS).
 Proof. 
   iSplit.
@@ -206,7 +121,156 @@ Proof.
       iRewrite - "H'" in "HσOS". by iRewrite "HσOS". 
 Qed.
 
-Lemma sem_row_filter_os {Σ} (ρ : sem_row Σ) `{ OSRow ρ } :
+Lemma row_tun_lookup {Σ} (ρ : sem_row Σ) (σ : sem_sig Σ) (l : label) (s : nat) :
+  (⦗ ρ | l ⦘%R !! (l, s) ≡ Some σ : iProp Σ) ⊣⊢
+  ∃ s', ⌜ s = S s' ⌝ ∗ (ρ !! (l, s') ≡ Some σ : iProp Σ).
+Proof. 
+  iSplit.
+  - iIntros "Hlookup".
+    destruct s.
+    + destruct (lookup_kmap_None (sem_row_tun_f l) ρ (l, 0)) as [_ H].
+      rewrite H; first (iDestruct "Hlookup" as "%H'"; inv H').
+      intros [l'' s''] H'. rewrite /sem_row_tun_f /= in H'.
+      destruct (decide (l = l'')) eqn:H''; inv H'.
+    + iExists s. iSplit; first done. 
+      replace (l, S s) with (sem_row_tun_f l (l, s)); last rewrite /sem_row_tun_f /= decide_True //.
+      rewrite lookup_kmap //. 
+  - iIntros "(%s' & -> & Hlookup)".
+    replace (l, S s') with (sem_row_tun_f l (l, s')); last rewrite /sem_row_tun_f /= decide_True //.
+    rewrite lookup_kmap //.
+Qed.
+
+Corollary row_tun_lookup_alt {Σ} (ρ : sem_row Σ) (σ : sem_sig Σ) (l : label) (s : nat) :
+  (⦗ ρ | l ⦘%R !! (l, S s) ≡ Some σ : iProp Σ) ⊣⊢
+  (ρ !! (l, s) ≡ Some σ : iProp Σ).
+Proof. 
+  iSplit. 
+  - rewrite row_tun_lookup. iIntros "(% & %Heq & H)".
+    by injection Heq as ->. 
+  - iIntros "H". 
+    iApply (row_tun_lookup ρ σ l (S s)). 
+    iExists s. eauto.
+Qed.
+
+Lemma row_tun_lookup_ne {Σ} (ρ : sem_row Σ) (σ : sem_sig Σ) (l l' : label) (s : nat) :
+  l ≠ l' →
+  (⦗ ρ | l' ⦘%R !! (l, s) ≡ Some σ : iProp Σ) ⊣⊢
+  (ρ !! (l, s) ≡ Some σ : iProp Σ).
+Proof. 
+  intros ?. 
+  assert (Heq : (l, s) = (sem_row_tun_f l' (l, s))).
+  { rewrite /sem_row_tun_f /= decide_False //. } 
+  iSplit; iIntros "Hlookup". 
+  - rewrite {1} Heq lookup_kmap //.
+  - rewrite {2} Heq lookup_kmap //.
+Qed.
+
+Lemma row_os_lookup {Σ} l s (σ : sem_sig Σ) (ρ : sem_row Σ) :
+  (¡ ρ)%R !! (l, s) ≡ Some σ ⊣⊢
+  ∃ (σ' : sem_sig Σ), σ ≡ (¡ σ')%S ∗ (ρ !! (l, s) ≡ Some σ' : iProp Σ).
+Proof. 
+  iSplit.
+  - rewrite lookup_fmap. iIntros "Hlookup".
+    destruct (ρ !! (l, s)) as [σ'|] eqn:H; rewrite H; simpl.
+    + iDestruct (option_equivI with "Hlookup") as "#Hlookup'".
+      iExists σ'. iSplit; last done.
+      by iRewrite - "Hlookup'".
+    + iDestruct "Hlookup" as "%H'". inv H'.
+  - iIntros "(%σ' & Heq & Hlookup)". rewrite lookup_fmap.
+    destruct (ρ !! (l, s)) as [σ''|] eqn:H; rewrite H; simpl.
+    + iDestruct (option_equivI with "Hlookup") as "#Hlookup'".
+      iRewrite "Hlookup'". by iRewrite "Heq".
+    + iDestruct "Hlookup" as "%H'". inv H'.
+Qed.
+
+Corollary row_os_lookup_alt {Σ} l s (σ : sem_sig Σ) (ρ : sem_row Σ) :
+  (ρ !! (l, s) ≡ Some σ : iProp Σ) ⊢
+  (¡ ρ)%R !! (l, s) ≡ Some (¡ σ)%S.
+Proof. 
+  iIntros "Hlookup". rewrite row_os_lookup.
+  iExists σ. by iFrame.
+Qed.
+
+(* One-Shot Rows *)
+
+Notation OSRow ρ := (MonoProt ⟦ ρ%R ⟧)%R.
+
+Global Instance row_nil_os_row {Σ} :
+  OSRow (⟨⟩ : sem_row Σ).
+Proof.
+  constructor. rewrite /sem_row_iEff /= /sem_row_nil.
+  iIntros (v Φ Φ') "_ (% & % & % & % & _ & H & _)".
+  rewrite lookup_empty. iDestruct "H" as "%". inv H. 
+Qed.
+  
+(* TODO: This needs to be generalised, 
+         if (l, 0) ∈ ρ then ρ(l, 0) does not need to be an OSSig.
+   NOTE: we can have a separate gset of keys that we don't need to check,
+         by creating a helper class *)
+Global Instance row_ins_os_row {Σ} (ρ : sem_row Σ) l (σ : sem_sig Σ) `{! OSSig σ, OSRow ρ } :
+  OSRow ((l, σ) · ρ).
+Proof.
+  constructor. iIntros (v Φ Φ') "HPost".
+  rewrite /sem_row_iEff /=.
+  iIntros "(%w & %l' & %s' & %σ' & -> & #Hlookup' & Hσ')".
+  destruct (decide ((l, 0) = (l', s'))). 
+  - rewrite /sem_row_ins. inv e. 
+    iExists w, l', 0, σ'. rewrite lookup_insert. 
+    iSplitR; first done. iFrame "#". 
+    iDestruct (option_equivI with "Hlookup'") as "#Hlookup''".
+    inv OSSig0. 
+    iDestruct (monotonic_prot with "HPost") as "H".
+    iDestruct (iEff_equivI σ.2 σ'.2) as "[Heq _]".
+    iSpecialize ("Heq" with "[]"); first by iRewrite "Hlookup''".
+    iRewrite - ("Heq" $! w Φ'). iApply "H". by iRewrite ("Heq" $! w Φ).
+  - inv OSRow0. rewrite /sem_row_iEff /= in monotonic_prot.
+    iDestruct (monotonic_prot (#(LitStr l'), #s', w)%V Φ Φ' with "HPost [Hσ']") as "(%w'' & %l'' & %s'' & %σ'' & %Heq & Hlookup & Hieff)".
+    { iExists w, l', s', σ'. iSplit; first done.
+      rewrite lookup_insert_ne; last done. iFrame "∗#". }
+    inv Heq. iExists w'', l'', s'', σ''. iSplitR; first done.
+    rewrite /sem_row_ins lookup_insert_ne; last done. iFrame "∗".
+Qed.
+
+Global Instance row_tun_os_row {Σ} (l : label) (ρ : sem_row Σ) `{ OSRow ρ } :
+  OSRow ⦗ ρ | l ⦘.
+Proof.
+  constructor. rewrite /sem_row_iEff /=. 
+  iIntros (v Φ Φ') "HPost".
+  iIntros "(%v' & %l' & %s' & %σ' & #Heq & #Hlookup & Hσ')".
+  destruct (decide (l = l')) as [->|Hll']. 
+  - iDestruct (row_tun_lookup with "Hlookup") as "(%s'' & -> & Hlookup')".
+    inv OSRow0.
+    iDestruct (monotonic_prot (effect l', #s'', v')%V Φ Φ' with "HPost [Hσ']") as "(%w & %l'' & %s''' & %σ'' & Heq' & Hlookup'' & Hσ'')".
+    { iExists v', l', s'', σ'. by iFrame "#∗". }
+    iExists v', l', (S s''), σ''. iDestruct "Heq'" as "%". inv H.
+    iFrame "#∗". iRewrite "Hlookup'" in "Hlookup''".
+    iDestruct (option_equivI with "Hlookup''") as "Heq'".
+    by iRewrite "Heq'" in "Hlookup". 
+  - rewrite (row_tun_lookup_ne ρ σ' l' l s'); last done.
+    inv OSRow0. rewrite /sem_row_iEff /= in monotonic_prot.
+    iDestruct (monotonic_prot (effect l', #s', v')%V Φ Φ' with "HPost [Hσ']") as "(%w & %l'' & %s'' & %σ'' & Heq' & Hlookup'' & Hσ'')".
+    { iExists v', l', s', σ'. by iFrame "#∗". }
+    iExists v', l', s', σ''. iDestruct "Heq'" as "%". inv H.
+    iRewrite "Heq"; iSplitR; first done. iFrame.
+    rewrite - (row_tun_lookup_ne ρ σ'' l'' l s'') //.
+Qed.
+
+Global Instance row_os_os_row {Σ} (ρ : sem_row Σ) :
+  OSRow (¡ ρ ).
+Proof.
+  constructor. rewrite /sem_row_iEff /=.
+  iIntros (v Φ Φ') "HPost (% & % & % & % & Heq & #Hlookup & Hσ)".
+  iExists v', l, s, σ. iFrame "∗#".
+  rewrite row_os_lookup. iDestruct "Hlookup" as "(%σ' & Heq & Hlookup)".
+  iDestruct (prod_equivI with "Heq") as "[_ Heq']". simpl.
+  iPoseProof (iEff_equivI with "Heq'") as "H".
+  iRewrite ("H" $! v' Φ'). 
+  pose proof (upcl_mono_prot σ'.2) as [].
+  iApply (monotonic_prot with "HPost").
+  by iRewrite - ("H" $! v' Φ).
+Qed.
+
+Lemma row_filter_os_os_row {Σ} (ρ : sem_row Σ) `{ OSRow ρ } :
   OSRow (filter_os ρ).
 Proof.
   constructor. iIntros (v Φ Φ') "HPost Hρ".
@@ -226,6 +290,20 @@ Proof.
   iRewrite "Heqσ". iFrame "#".
 Qed.
 
+Lemma os_row_mono_prot {Σ} (ρ : sem_row Σ) l s (σ : sem_sig Σ) `{ OSRow ρ } :
+  ρ !! (l, s) ≡ Some σ -∗ mono_prot σ.2.
+Proof.
+  inv OSRow0.
+  iIntros "#Hlookup % % % HPost Hσ". 
+  iDestruct (monotonic_prot (effect l, #s, v)%V Φ Φ' with "HPost") as "H".
+  iDestruct ("H" with "[Hσ]") as "H".
+  { iExists v, l, s, σ. by iFrame "#∗". }
+  iDestruct "H" as "(%v' & %l' & %s' & %σ' & %Heq & Hlookup' & Hσ')".
+  inv Heq. destruct (ρ !! (l', s')) eqn:Heq; last (iDestruct "Hlookup'" as "%H"; inv H).
+  rewrite Heq !option_equivI. iRewrite "Hlookup'" in "Hlookup".
+  rewrite prod_equivI_2 iEff_equivI.
+  by iRewrite ("Hlookup" $! v' Φ') in "Hσ'".
+Qed.
 
 (* Subsumption relation on rows *)
 
@@ -298,30 +376,7 @@ Proof.
   iExists σ. iFrame "#". iApply sig_le_refl.
 Qed.
 
-Lemma row_tun_ins {Σ} l s σ (ρ : sem_row Σ) :
-  (⦗ insert (l, s) σ ρ | l ⦘ = insert (l, S s) σ ⦗ ρ | l ⦘)%R. 
-Proof.
-  rewrite {1} /sem_row_tun /=. 
-  rewrite (kmap_insert _ ρ (l, s) σ) // {1}/sem_row_tun_f /= decide_True //.
-Qed.
-
-Lemma row_tun_ins_ne {Σ} l l' s σ (ρ : sem_row Σ) :
-  l ≠ l' →
-  (⦗ insert (l, s) σ ρ | l' ⦘ = insert (l, s) σ ⦗ ρ | l' ⦘)%R. 
-Proof.
-  intros ?. rewrite {1} /sem_row_tun /=. 
-  rewrite (kmap_insert _ ρ (l, s) σ) // {1}/sem_row_tun_f /= decide_False //.
-Qed.
-
-Lemma row_os_ins_gen {Σ} l s σ (ρ : sem_row Σ) :
-  (¡ (insert (l, s) σ ρ))%R = insert (l, s) (¡ σ)%S (¡ ρ)%R.
-Proof. rewrite /sem_row_os fmap_insert //. Qed.
-
-Corollary row_os_ins {Σ} l σ (ρ : sem_row Σ) :
-  (¡ ((l, σ) · ρ))%R = ((l, ¡ σ)%S · (¡ ρ))%R.
-Proof. apply row_os_ins_gen. Qed.
-
-Lemma row_le_ins_comp {Σ} (ρ ρ' : sem_row Σ) (l : string) (σ σ' : sem_sig Σ) : 
+Lemma row_le_ins_comp {Σ} (ρ ρ' : sem_row Σ) (l : label) (σ σ' : sem_sig Σ) : 
   ρ ≤R ρ' -∗ σ ≤S σ' -∗
   (l, σ) · ρ ≤R (l, σ') · ρ'.
 Proof.
@@ -344,7 +399,7 @@ Proof.
     iFrame "#".
 Qed.
 
-Lemma row_le_ins {Σ} (ρ : sem_row Σ) (l : string) (σ : sem_sig Σ) : 
+Lemma row_le_ins {Σ} (ρ : sem_row Σ) (l : label) (σ : sem_sig Σ) : 
   ρ !! (l, 0) ≡ None -∗
   ρ ≤R (l, σ) · ρ. 
 Proof. 
@@ -359,44 +414,148 @@ Proof.
     iFrame "#". iApply sig_le_refl.
 Qed.
 
-Lemma row_le_ins_tun {Σ} (ρ : sem_row Σ) (l : string) (σ : sem_sig Σ) : 
-  ⊢ ⦗ ρ ⦘ ≤R (l, σ) · ⦗ ρ ⦘. 
+Lemma row_le_ins_tun {Σ} (ρ : sem_row Σ) (l : label) (σ : sem_sig Σ) : 
+  ⊢ ⦗ ρ | l ⦘ ≤R (l, σ) · ⦗ ρ | l ⦘. 
 Proof. 
   iApply row_le_ins. rewrite /sem_row_tun.
-  pose proof (lookup_kmap_None sem_row_tun_f ρ (l, 0)) as [_ H].
+  pose proof (lookup_kmap_None (sem_row_tun_f l) ρ (l, 0)) as [_ H].
   rewrite H; first done.
-  intros i Hlookup. inv Hlookup.
+  intros i Hlookup. rewrite /sem_row_tun_f in Hlookup.
+  destruct (decide (l = i.1)); inv Hlookup.
 Qed.
 
-Lemma row_le_tun_comp {Σ} (ρ ρ' : sem_row Σ) :
+Lemma row_le_tun_comp {Σ} (l : label) (ρ ρ' : sem_row Σ) :
   ρ ≤R ρ' -∗
-  ⦗ ρ ⦘ ≤R ⦗ ρ' ⦘. 
+  ⦗ ρ | l ⦘ ≤R ⦗ ρ' | l ⦘. 
 Proof. 
-  iIntros "Hle %l %s %σ Hlookup".
-  destruct s.
-  - destruct (lookup_kmap_None sem_row_tun_f ρ (l, 0)) as [_ H].
-    rewrite H; first (iDestruct "Hlookup" as "%H'"; inv H').
-    intros [l' s'] H'. inv H'. 
-  - rewrite /sem_row_tun.
-    assert (Heq : (l, S s) = (sem_row_tun_f (l, s))) by done.
-    rewrite Heq !lookup_kmap.
-    by iApply "Hle".
+  iIntros "Hle %l' %s' %σ' Hlookup".
+  Search "∗-∗".
+  destruct (decide (l = l')) as [->|Hneq].
+  - rewrite (row_tun_lookup ρ σ' l' s'). 
+    iDestruct "Hlookup" as "(%s'' & -> & Hlookup)".
+    iDestruct ("Hle" with "Hlookup") as (σ'') "[H H']".
+    iExists σ''. iFrame. 
+    rewrite - (row_tun_lookup_alt ρ' σ'' l' s'') //. 
+  - rewrite (row_tun_lookup_ne); last done.
+    iDestruct ("Hle" with "Hlookup") as (σ'') "[H H']".
+    iExists σ''. rewrite row_tun_lookup_ne; last done. iFrame.
 Qed.
+
+Lemma row_tun_ins_eq {Σ} l s σ (ρ : sem_row Σ) :
+  (⦗ insert (l, s) σ ρ | l ⦘ = insert (l, S s) σ ⦗ ρ | l ⦘)%R. 
+Proof.
+  rewrite {1} /sem_row_tun /=. 
+  rewrite (kmap_insert _ ρ (l, s) σ) // {1}/sem_row_tun_f /= decide_True //.
+Qed.
+
+Lemma row_tun_ins_eq_ne {Σ} l l' s σ (ρ : sem_row Σ) :
+  l ≠ l' →
+  (⦗ insert (l, s) σ ρ | l' ⦘ = insert (l, s) σ ⦗ ρ | l' ⦘)%R. 
+Proof.
+  intros ?. rewrite {1} /sem_row_tun /=. 
+  rewrite (kmap_insert _ ρ (l, s) σ) // {1}/sem_row_tun_f /= decide_False //.
+Qed.
+
+Corollary row_le_tun_ins_ne {Σ} l l' σ (ρ : sem_row Σ) :
+  l ≠ l' →
+  ⊢ ⦗ (l, σ) · ρ | l' ⦘ ≤R (l, σ) · ⦗ ρ | l' ⦘.
+Proof.
+  intros ?. rewrite row_tun_ins_eq_ne; last done.
+  iApply row_le_refl.
+Qed.
+
+Corollary row_le_ins_tun_ne {Σ} l l' σ (ρ : sem_row Σ) :
+  l ≠ l' →
+  ⊢ (l, σ) · ⦗ ρ | l' ⦘ ≤R ⦗ (l, σ) · ρ | l' ⦘.
+Proof.
+  intros ?. rewrite row_tun_ins_eq_ne; last done.
+  iApply row_le_refl.
+Qed.
+
+Lemma row_le_tun_comm {Σ} l l' (ρ : sem_row Σ) :
+  ⊢ ⦗ ⦗ ρ | l ⦘ | l' ⦘ ≤R ⦗ ⦗ ρ | l' ⦘ | l ⦘.
+Proof. 
+  iIntros (l'' s'' σ'') "Hlookup".
+  destruct (decide (l' = l'')) as [->|H].
+  - rewrite row_tun_lookup. iDestruct "Hlookup" as "(%si'' & -> & Hlookup)".
+    destruct (decide (l = l'')) as [->|H].
+    + rewrite row_tun_lookup. iDestruct "Hlookup" as "(%s & -> & Hlookup)".
+      iExists σ''. rewrite ! row_tun_lookup_alt. iSplit; [done|iApply sig_le_refl].
+    + rewrite row_tun_lookup_ne; last done. 
+      iExists σ''. rewrite row_tun_lookup_ne; last done.
+      rewrite row_tun_lookup_alt. iFrame. iApply sig_le_refl.
+  - rewrite row_tun_lookup_ne; last done. 
+    destruct (decide (l = l'')) as [->|].
+    + rewrite row_tun_lookup. iDestruct "Hlookup" as "(%si'' & -> & Hlookup)".
+      iExists σ''. rewrite row_tun_lookup_alt.
+      rewrite row_tun_lookup_ne; last done. iFrame. iApply sig_le_refl.
+    + rewrite row_tun_lookup_ne; last done.
+      iExists σ''. do 2 (rewrite row_tun_lookup_ne; try done).
+      iFrame. iApply sig_le_refl.
+Qed.
+
+Lemma row_os_ins_eq {Σ} l s σ (ρ : sem_row Σ) :
+  (¡ (insert (l, s) σ ρ))%R = insert (l, s) (¡ σ)%S (¡ ρ)%R.
+Proof. rewrite /sem_row_os fmap_insert //. Qed.
+
+Corollary row_le_os_ins {Σ} l σ (ρ : sem_row Σ) :
+  ⊢ ¡ ((l, σ) · ρ) ≤R (l, ¡ σ)%S · (¡ ρ).
+Proof. rewrite row_os_ins_eq /=. iApply row_le_refl. Qed.
+
+Corollary row_le_ins_os {Σ} l σ (ρ : sem_row Σ) :
+   ⊢ (l, ¡ σ)%S · (¡ ρ) ≤R ¡ ((l, σ) · ρ).
+Proof. rewrite row_os_ins_eq /=. iApply row_le_refl. Qed.
 
 Lemma row_le_os_comp {Σ} (ρ ρ' : sem_row Σ) :
   ρ ≤R ρ' -∗
   ¡ ρ ≤R ¡ ρ'. 
-Proof. Admitted.
+Proof. 
+  iIntros "Hle %l %s %σ #Hlookup".
+  rewrite row_os_lookup. iDestruct "Hlookup" as "(%σ1 & Heq & Hlookup)".
+  iDestruct ("Hle" $! l s with "Hlookup") as "(%σ' & #Hlookup' & #Hle)".
+  iExists (¡ σ')%S. rewrite row_os_lookup. iSplit. 
+  { iExists σ'. iSplit; by iFrame. }
+  iRewrite "Heq". by iApply sig_le_os_comp.
+Qed.
   
-Lemma row_le_os_intro {Σ} (ρ : sem_row Σ) `{OSRow ρ} :
+Lemma row_le_os_intro {Σ} (ρ : sem_row Σ) :
   ⊢ ρ ≤R ¡ ρ. 
-Proof. Admitted.
+Proof. 
+  iIntros (l s σ) "#Hlookup".
+  iExists (¡ σ)%S. rewrite row_os_lookup. 
+  iSplit; last iApply sig_le_os_intro.
+  iExists σ. by iFrame "#".
+Qed.
 
-Lemma row_le_os_elim {Σ} (ρ : sem_row Σ) :
+Lemma row_le_os_elim {Σ} (ρ : sem_row Σ) `{OSRow ρ}:
   ⊢ ¡ ρ ≤R ρ. 
-Proof. Admitted.
+Proof. 
+  iIntros (l s σ) "#Hlookup".
+  rewrite row_os_lookup. iDestruct "Hlookup" as "(%σ' & Heq & Hlookup)".
+  iExists σ'. iFrame "#". iRewrite "Heq". 
+  iPoseProof (os_row_mono_prot with "Hlookup") as "Hmono". 
+  iDestruct (prod_equivI with "Heq") as "[Heqm _]". simpl.
+  (* We can't use sig_le_os_elim here because it requires OSSig σ
+   * which leaves outside the current iProp context. 
+   * Instead we have to prove it directly *)
+  iSplit; first (iRewrite "Heqm"; iApply mode_le_refl).
+  iIntros (v Φ) "!# Hσ'".  iDestruct "Hσ'" as "(%Φ' & Hσ' & HPost)".
+  by iApply ("Hmono" with "HPost").
+Qed.
 
-Lemma row_le_swap_second {Σ} (l l' : string) (σ σ' : sem_sig Σ) (ρ : sem_row Σ) : 
+Lemma row_os_tun_eq {Σ} l (ρ : sem_row Σ) :
+  (⦗ (¡ ρ) | l ⦘ = ¡ ⦗ ρ | l ⦘)%R. 
+Proof. rewrite /sem_row_tun /sem_row_os /= kmap_fmap //. Qed.
+
+Corollary row_le_tun_os {Σ} (l : label) (ρ : sem_row Σ) :
+  ⊢ ⦗ (¡ ρ) | l ⦘ ≤R ¡ ⦗ ρ | l ⦘. 
+Proof. rewrite row_os_tun_eq. iApply row_le_refl. Qed.
+
+Corollary row_le_os_tun {Σ} (l : label) (ρ : sem_row Σ) :
+  ⊢  ¡ ⦗ ρ | l ⦘ ≤R ⦗ (¡ ρ) | l ⦘.
+Proof. rewrite row_os_tun_eq. iApply row_le_refl. Qed.
+
+Lemma row_le_swap_second {Σ} (l l' : label) (σ σ' : sem_sig Σ) (ρ : sem_row Σ) : 
   l ≠ l' →
   ⊢ (l, σ) · (l', σ') · ρ ≤R (l', σ') · (l, σ) · ρ. 
 Proof. 
@@ -405,7 +564,7 @@ Proof.
   intros ?. inv H.
 Qed.
 
-Lemma row_le_swap_third {Σ} (l l' l'' : string) (σ σ' σ'' : sem_sig Σ) (ρ : sem_row Σ) : 
+Lemma row_le_swap_third {Σ} (l l' l'' : label) (σ σ' σ'' : sem_sig Σ) (ρ : sem_row Σ) : 
   l ≠ l' → l' ≠ l'' → l'' ≠ l →
   ⊢ (l, σ) · (l', σ') · (l'', σ'') · ρ ≤R 
     (l'', σ'') · (l, σ) · (l', σ') · ρ. 
@@ -415,7 +574,7 @@ Proof.
   iApply row_le_refl. 
 Qed.
 
-Lemma row_le_swap_fourth {Σ} (l l' l'' l''' : string) (σ σ' σ'' σ''': sem_sig Σ) (ρ : sem_row Σ) : 
+Lemma row_le_swap_fourth {Σ} (l l' l'' l''' : label) (σ σ' σ'' σ''': sem_sig Σ) (ρ : sem_row Σ) : 
   l ≠ l' → l ≠ l'' → l ≠ l''' → l' ≠ l'' → l' ≠ l''' → l'' ≠ l''' → 
   ⊢ (l, σ) · (l', σ') · (l'', σ'') · (l''', σ''') · ρ ≤R 
     (l''', σ''') · (l, σ) · (l', σ') · (l'', σ'') · ρ.
