theories/lang/handler.v
@@ -1,0 +1,331 @@
+
+(* handler.v *)
+
+(* This file defines the Haffel handlers. *)
+
+From iris.algebra Require Import ofe.
+From iris.base_logic Require Export lib.iprop .
+From iris.program_logic Require Export language.
+From iris.proofmode Require Import base tactics classes.
+From iris.heap_lang Require Export locations.
+
+(* Hazel language *)
+From hazel.language Require Export eff_lang.
+From hazel.program_logic Require Import weakest_precondition 
+                                        basic_reasoning_rules
+                                        deep_handler_reasoning
+                                        tactics
+                                        shallow_handler_reasoning
+                                        state_reasoning.
+
+From haffel.lib Require Export base logic.
+
+Definition rec_perform : val := (λ: "x", "x")%V.
+
+Notation "'perform:' ( l , e )" := (rec_perform (Do OS ((l, #0)%V, e%E)))%E
+  (at level 200, e at level 200,
+   format "'[' 'perform:' ( l , e ) ']'") : expr_scope.
+
+Notation "'performₘ:' ( l , e )" := (rec_perform (Do MS ((l, #0)%V, e%E)))%E
+  (at level 200, e at level 200,
+   format "'[' 'performₘ:' ( l , e ) ']'") : expr_scope.
+
+Notation "'effect' l" := (#(LitStr l))%V (at level 70) : val_scope.
+Notation label := (string).
+
+Definition shallow_try_mode : val := (
+  λ: "e" "hos" "hms" "r",
+    shallow-try: "e" #() with
+      effect (λ: "x" "k", 
+          if: UnOp IsContOS "k" then
+            "hos" "x" "k"
+          else
+            "hms" "x" "k"
+      )
+    | return "r" 
+    end
+)%V.
+
+Arguments shallow_try_mode : simpl never.
+
+Definition ShallowTryMode (e : expr) (hos hms r : expr) : expr :=
+  shallow_try_mode (λ: <>, e)%E hos hms r.
+
+Definition ShallowTryModeV (e : expr) (hos hms r : expr) : expr :=
+  shallow_try_mode (λ: <>, e)%V hos hms r.
+
+Notation "'shallow-try-mode:' e 'with' 'effect-os' hos | 'effect-ms' hms | 'return' r 'end'" :=
+  (ShallowTryMode e hos hms r)
+  (e, hos, hms, r at level 200, only parsing) : expr_scope.
+
+Definition deep_try_mode : val := (
+    rec: "H" "e" "hos" "hms" "r" := 
+      ShallowTryMode ("e" #())
+        (λ: "x" "k", "hos" "x" (λ: "y", "H" (λ: <>, "k" "y") "hos" "hms" "r"))
+        (λ: "x" "k", "hms" "x" (λ: "y", "H" (λ: <>, "k" "y") "hos" "hms" "r"))
+        "r"
+)%V.
+
+Arguments deep_try_mode : simpl never.
+
+Definition DeepTryMode (e : expr) (hos hms r : expr) : expr :=
+  deep_try_mode (λ: <>, e)%E hos hms r.
+
+Definition DeepTryModeV (e : expr) (hos hms r : expr) : expr :=
+  deep_try_mode (λ: <>, e)%V hos hms r.
+
+Notation "'deep-try-mode:' e 'with' 'effect-os' hos | 'effect-ms' hms | 'return' r 'end'" :=
+  (DeepTryMode e hos hms r)
+  (e, hos, hms, r at level 200, only parsing) : expr_scope.
+
+
+Definition shallow_handler_mode `{irisGS eff_lang Σ}
+  (E : coPset)
+  (Ψ1 : iEff Σ)
+  (Ψ2 : iEff Σ)
+  (Φ : val -d> iPropO Σ)
+  (hos hms r : val)
+  (Ψ1' : iEff Σ)
+  (Ψ2' : iEff Σ)
+  (Φ' : val -d> iPropO Σ) : iProp Σ :=
+
+  (* Correctness of the return branch. *)
+  (∀ (y : val), Φ y -∗ EWP r y @ E <| Ψ1' |> {| Ψ2' |} {{ Φ' }}) ∧
+
+  (* Correctness of the effect one-shot branch. *)
+  (∀ (v k : val),
+     iEff_car (upcl OS Ψ1) v (λ w, EWP k w @ E <| Ψ1 |> {| Ψ2 |} {{ Φ }}) -∗
+       EWP hos v k @ E <| Ψ1' |> {| Ψ2' |} {{ Φ' }}) ∧
+
+  (* Correctness of the effect multi-shot branch. *)
+  (∀ (v k : val),
+     iEff_car (upcl MS Ψ2) v (λ w, EWP k w @ E <| Ψ1 |> {| Ψ2 |} {{ Φ }}) -∗
+       EWP hms v k @ E <| Ψ1' |> {| Ψ2' |} {{ Φ' }}).
+
+Lemma ewp_try_with_mode `{heapGS Σ} E e Ψ1 Ψ2 Φ (hos hms r : val) Ψ1' Ψ2' Φ' : 
+  EWP e @ E <| Ψ1 |> {| Ψ2 |} {{ Φ }} -∗
+    shallow_handler_mode E Ψ1 Ψ2 Φ hos hms r Ψ1' Ψ2' Φ' -∗
+      EWP (ShallowTryModeV e hos hms r) @ E <| Ψ1' |> {| Ψ2' |} {{ Φ' }}.
+Proof.
+  iIntros "He H". rewrite /ShallowTryModeV /shallow_try_mode /shallow_handler_mode. 
+  ewp_pure_steps. 
+  iApply (ewp_try_with with "[He] [H]").
+  { ewp_pure_steps. iApply "He". }
+  iSplit; last iSplit.
+  - iDestruct "H" as "[$ _]". 
+  - iIntros (v k) "(%N & %l & ->) HΨ1". 
+    iDestruct "H" as "[_ [H _]]". 
+    ewp_pure_steps; first done. ewp_pure_steps.
+    by iApply "H". 
+  - iIntros (v k) "(%N & ->) HΨ1". 
+    iDestruct "H" as "[_ [_ H]]". 
+    ewp_pure_steps; first done. ewp_pure_steps.
+    by iApply "H". 
+Qed.
+
+Notation deep_handler_mode_type Σ :=
+  (coPset -d> iEff Σ -d> iEff Σ -d> (val -d> iPropO Σ) 
+         -d> val -d> val -d> val 
+         -d> iEff Σ -d> iEff Σ -d> (val -d> iPropO Σ) -d> iPropO Σ) (only parsing).
+
+Definition deep_handler_mode_pre `{irisGS eff_lang Σ} :
+  deep_handler_mode_type Σ → deep_handler_mode_type Σ :=
+  (λ deep_handler_mode E Ψ1 Ψ2 Φ hos hms r Ψ1' Ψ2' Φ', 
+
+  (* Correctness of the return branch. *)
+  (∀ (y : val), Φ y -∗ EWP r y @ E <| Ψ1' |> {| Ψ2' |} {{ Φ' }}) ∧
+
+  (* Correctness of the effect one-shot branch. *)
+  (∀ (v k : val),
+     iEff_car (upcl OS Ψ1) v (λ w, 
+      ∀ Ψ1'' Ψ2'' Φ'',
+        ▷ deep_handler_mode E Ψ1 Ψ2 Φ hos hms r Ψ1'' Ψ2'' Φ'' -∗
+        EWP k w @ E <| Ψ1'' |> {| Ψ2'' |} {{ Φ'' }}) -∗
+       EWP hos v k @ E <| Ψ1' |> {| Ψ2' |} {{ Φ' }}) ∧
+
+  (* Correctness of the effect multi-shot branch. *)
+  (∀ (v k : val),
+     iEff_car (upcl MS Ψ2) v (λ w, 
+      ∀ Ψ1'' Ψ2'' Φ'',
+        ▷ deep_handler_mode E Ψ1 Ψ2 Φ hos hms r Ψ1'' Ψ2'' Φ'' -∗
+        EWP k w @ E <| Ψ1'' |> {| Ψ2'' |} {{ Φ'' }}) -∗
+       EWP hms v k @ E <| Ψ1' |> {| Ψ2' |} {{ Φ' }}))%I.
+
+Local Instance deep_handler_mode_pre_contractive `{heapGS Σ} : Contractive deep_handler_mode_pre.
+Proof.
+  rewrite /deep_handler_mode_pre => n deep deep' Hne E Ψ1 Ψ2 Φ h r Ψ1' Ψ2' Φ'.
+  repeat (f_contractive || f_equiv). intros ?; simpl.
+  repeat (f_contractive || f_equiv); apply Hne.
+Qed.
+Definition deep_handler_mode `{heapGS Σ} := fixpoint deep_handler_mode_pre.
+Arguments deep_handler_mode _ _%ieff _%ieff _%I _%V %V _%V _%ieff _%ieff _%I.
+
+Global Lemma deep_handler_mode_unfold `{heapGS Σ} E Ψ1 Ψ2 Φ hos hms r Ψ1' Ψ2' Φ' :
+  deep_handler_mode E Ψ1 Ψ2 Φ hos hms r Ψ1' Ψ2' Φ' ⊣⊢
+    deep_handler_mode_pre deep_handler_mode E Ψ1 Ψ2 Φ hos hms r Ψ1' Ψ2' Φ'.
+Proof.
+  by apply (fixpoint_unfold deep_handler_mode_pre).
+Qed.
+
+Lemma ewp_deep_try_with_mode `{heapGS Σ} E e Ψ1 Ψ2 Φ (hos hms r : val) Ψ1' Ψ2' Φ' : 
+  EWP e @ E <| Ψ1 |> {| Ψ2 |} {{ Φ }} -∗
+    deep_handler_mode E Ψ1 Ψ2 Φ hos hms r Ψ1' Ψ2' Φ' -∗
+      EWP (DeepTryModeV e hos hms r) @ E <| Ψ1' |> {| Ψ2' |} {{ Φ' }}.
+Proof.
+  iIntros "He H". rewrite /DeepTryModeV /deep_try_mode.
+  iLöb as "IH" forall (e Ψ1' Ψ2' Φ'). ewp_pure_steps.
+  rewrite deep_handler_mode_unfold /deep_handler_mode_pre.
+  iApply (ewp_try_with_mode with "[He] [H]").
+  { ewp_pure_steps. iApply "He". }
+  iSplit; last iSplit.
+  - iDestruct "H" as "[$ _]". 
+  - iIntros (v k) "/= (%Φ'' & HΨ1 & HPost)". 
+    iDestruct "H" as "[_ [H _]]".
+    ewp_pure_steps. iApply "H". iExists Φ''. iFrame.
+    iIntros (w) "HΦ'' % % %Φ''' Hdeep".
+    do 3 ewp_value_or_step.
+    iApply ("IH" with "[HΦ'' HPost] Hdeep"); by iApply "HPost".
+  - iIntros (v k) "/= (%Φ'' & HΨ2 & #HPost)".
+    iDestruct "H" as "[_ [_ H]]".
+    ewp_pure_steps. iApply "H". iExists Φ''. iFrame.
+    iIntros (w) "!# HΦ'' % % %Φ''' Hdeep".
+    do 3 ewp_value_or_step.
+    iApply ("IH" with "[HΦ'' HPost] Hdeep"); by iApply "HPost".
+Qed.
+
+Definition shallow_try_eff : label → val → val → val → mode → val := λ l' h r H m, 
+      (λ: "x" "k",
+          let: "l" := Fst (Fst "x") in
+          let: "s" := Snd (Fst "x") in
+          let: "x" := Snd "x" in
+          if: ("l" = (effect l')%V) && ("s" = #0) then
+            h "x" "k"
+          else
+            (λ: "y", H (λ: <>, "k" "y") (effect l')%V h r) (Do m ("l", "s", "x"))
+      )%V.
+
+Definition shallow_try_ls : val := (
+  rec: "H" "e" "l'" "h" "r" :=
+    shallow_try_mode "e" 
+      (λ: "x" "k",
+          let: "l" := Fst (Fst "x") in
+          let: "s" := Snd (Fst "x") in
+          let: "x" := Snd "x" in
+          if: ("l" = "l'") && ("s" = #0) then
+            "h" "x" "k"
+          else
+            (λ: "y", "H" (λ: <>, "k" "y") "l'" "h" "r") (Do OS ("l", "s", "x"))
+      )%E
+      (λ: "x" "k",
+          let: "l" := Fst (Fst "x") in
+          let: "s" := Snd (Fst "x") in
+          let: "x" := Snd "x" in
+          if: ("l" = "l'") && ("s" = #0) then
+            "h" "x" "k"
+          else
+            (λ: "y", "H" (λ: <>, "k" "y") "l'" "h" "r") (Do MS ("l", "s", "x"))
+      )%E
+      "r"
+)%V.
+
+Arguments shallow_try_ls : simpl never.
+
+Definition ShallowTryLS (e : expr) (l : label) (h r : expr) : expr :=
+  shallow_try_ls (λ: <>, e)%E (effect l)%V h r.
+
+Definition ShallowTryLSV (e : expr) (l : label) (h r : expr) : expr :=
+  shallow_try_ls (λ: <>, e)%V (effect l)%V h r.
+
+Notation "'shallow-try-ls:' e 'handle' l 'with' 'effect' h | 'return' r 'end'" :=
+  (ShallowTryLS e l h r)
+  (e, l, h, r at level 200, only parsing) : expr_scope.
+
+Definition deep_try_ls : val := (
+  λ: "e" "l'" "h" "r",
+    deep_try_mode "e"
+      (λ: "x" "k", 
+          let: "l" := Fst (Fst "x") in
+          let: "s" := Snd (Fst "x") in
+          let: "x" := Snd "x" in
+          if: ("l" = "l'") && ("s" = #0) then
+            "h" "x" "k"
+          else
+            "k" (Do OS ("l", "s", "x"))
+      )
+      (λ: "x" "k", 
+          let: "l" := Fst (Fst "x") in
+          let: "s" := Snd (Fst "x") in
+          let: "x" := Snd "x" in
+          if: ("l" = "l'") && ("s" = #0) then
+            "h" "x" "k"
+          else
+            "k" (Do MS ("l", "s", "x"))
+      )
+      "r" 
+)%V.
+            
+Arguments deep_try_ls : simpl never.
+
+Definition DeepTryLS (e : expr) (l : label) (h r : expr) : expr :=
+  deep_try_ls (λ: <>, e)%E (effect l)%V h r.
+
+Definition DeepTryLSV (e : expr) (l : label) (h r : expr) : expr :=
+  deep_try_ls (λ: <>, e)%V (effect l)%V h r.
+
+Notation "'deep-try-ls:' e 'handle' l 'with' 'effect' h | 'return' r 'end'" :=
+  (DeepTryLS e l h r)
+  (e, l, h, r at level 200, only parsing) : expr_scope.
+
+Definition lft_def : val := 
+  (λ: "l'" "e", 
+     deep-try-mode: "e" #() with
+       effect-os (λ: "x" "k", 
+             let: "l" := Fst (Fst "x") in
+             let: "s" := Snd (Fst "x") in
+             let: "x" := Snd "x" in
+             if: "l" = "l'" then
+               "k" (Do OS ("l", "s" + #1, "x"))
+             else
+               "k" (Do OS ("l", "s", "x"))
+         )
+       | effect-ms (λ: "x" "k", 
+             let: "l" := Fst (Fst "x") in
+             let: "s" := Snd (Fst "x") in
+             let: "x" := Snd "x" in
+             if: "l" = "l'" then
+               "k" (Do MS ("l", "s" + #1, "x"))
+             else
+               "k" (Do MS ("l", "s", "x"))
+         )
+       | return (λ: "x", "x")%V 
+      end
+)%V.
+
+Notation "'lft:' ( l , e )" := (lft_def l%V (λ: <>, e)%E) (at level 10) : expr_scope.
+
+Definition unlft_def : val := 
+  (λ: "l'" "e", 
+     deep-try-mode: "e" #() with
+       effect-os (λ: "x" "k", 
+             let: "l" := Fst (Fst "x") in
+             let: "s" := Snd (Fst "x") in
+             let: "x" := Snd "x" in
+             if: "l" = "l'" then
+               "k" (Do OS ("l", "s" - #1, "x"))
+             else
+               "k" (Do OS ("l", "s", "x"))
+         )
+       | effect-ms (λ: "x" "k", 
+             let: "l" := Fst (Fst "x") in
+             let: "s" := Snd (Fst "x") in
+             let: "x" := Snd "x" in
+             if: "l" = "l'" then
+               "k" (Do MS ("l", "s" - #1, "x"))
+             else
+               "k" (Do MS ("l", "s", "x"))
+         )
+       | return (λ: "x", "x")%V 
+      end
+)%V.
+
+Notation "'unlft:' ( l , e )" := (unlft_def l%V (λ: <>, e)%E) (at level 10) : expr_scope.
