theories/lang/iEff.v
@@ -2,8 +2,8 @@
 From iris.proofmode  Require Import tactics.
 From iris.base_logic Require Export lib.iprop.
 
+From hazel.language Require Export eff_lang.
 From hazel.program_logic Require Export protocols.
-From haffel.lang Require Import haffel.
 
 Lemma iEff_tele_eq' {Σ} (TT1 TT2 : tele) v m
   (v' : TT1 -t>         val) (P : TT1 -t>         iProp Σ)
@@ -20,4 +20,19 @@ Proof.
   by rewrite (iEff_tele_eq (tele_app v') (tele_app P)
                   (λ x y, tele_app (tele_app w' x) y)
                   (λ x y, tele_app (tele_app Q  x) y)).
+Qed.
+
+Lemma iEff_le_upcl_intro {Σ} m (Ψ : iEff Σ) :
+  ⊢ iEff_le Ψ (upcl m Ψ). 
+Proof.
+  iIntros (v Φ) "!# HΨ". iExists Φ. iFrame.
+  destruct m; simpl; [iIntros "% $"|iIntros "!# % $"].
+Qed.
+
+Lemma iEff_le_upcl_ms_os {Σ} (Ψ : iEff Σ) :
+  ⊢ iEff_le (upcl MS Ψ) (upcl OS Ψ).
+Proof.
+  iIntros (v Φ) "!# HMSΨ". rewrite /upcl /=.
+  iDestruct "HMSΨ" as "(%Φ' & HΨΦ' & #HPost)".
+  iExists Φ'. iFrame "#∗".
 Qed.
