theories/logic/copyable.v
@@ -16,7 +16,6 @@ From hazel.program_logic Require Import weakest_precondition
 
 (* Local imports *)
 From haffel.lang Require Import haffel.
-From haffel.lang Require Import subst_map.
 From haffel.logic Require Import sem_def.
 From haffel.logic Require Import sem_sig.
 From haffel.logic Require Import sem_types.
